base/lambda_star_overlap_prop_set/lambda_star.v
@@ -1,0 +1,1944 @@
+Require Export Arith.EqNat.
+Require Export Arith.Le.
+Require Import Coq.Arith.Arith.
+Require Import Coq.Bool.Bool.
+Require Import Coq.Program.Equality.
+Require Import Coq.Lists.List.
+Require Import Psatz.
+Require Import ZArith.
+Require Import Coq.Arith.Compare_dec.
+Import ListNotations.
+
+Require Import nats.
+Require Import vars.
+Require Import env.
+Require Import tactics.
+Require Import qualifiers.
+
+Import QualNotations.
+Local Open Scope qualifiers.
+
+Require Import FunctionalExtensionality.
+Require Import Coq.Logic.PropExtensionality.
+
+Definition id := nat.
+
+Definition lt_S_n :=
+  fun n m : nat => proj2 (Nat.succ_lt_mono n m).
+Definition le_plus_r := 
+  fun n m : nat => Nat.le_add_l m n.
+
+(* Definitions *)
+
+(* ### Syntax ### *)
+(* We represent terms and types in locally nameless style. *)
+
+(* Types *)
+Inductive ty : Type :=
+| TUnit : ty                             (* Unit base type*)
+| TFun  : qual -> qual -> ty -> ty -> ty (* Dependent function type TFun q1 q2 T1 T2 ~> ((x: T1^q1) => T2^q2),
+                                            where x is bound in T2 and q2.
+                                            Bound variables are represented by de Bruijn indices, where x ~> #0. *)
+| TRef  : ty -> ty                       (* Mutable reference type TRef T ~> Ref[T]. *)
+.
+
+(* Terms *)
+Inductive tm : Type :=
+| tunit   : tm              (* The unit value. *)
+| tvar    : var -> tm       (* Term variable, either free (tvar $n) (de Bruijn level), or bound (tvar #n) (de Bruijn index). *)
+| tabs    : tm  -> tm       (* Lambda abstractions (tabs t) ~> λx.t, where x ~> #0. *)
+| tapp    : tm  -> tm -> tm (* Function application. *)
+| tloc    : loc -> tm       (* A store location literal. *)
+| tref    : tm  -> tm       (* Reference allocation (tref t) ~> new Ref(t). *)
+| tderef  : tm  -> tm       (* Dereference (tderef t) ~> !t. *)
+| tassign : tm  -> tm -> tm (* Reference assignment (tassign t1 t2) ~> t1 := t2. *)
+.
+
+Notation "& l" := (tloc l) (at level 0).
+Notation "! t" := (tderef t) (at level 0).
+Coercion tvar : var >-> tm. (* lightens the notation of term variables *)
+
+Definition tenv := list (ty * qual).
+Definition senv := list ty. (* Sigma store typing *)
+
+#[global] Hint Rewrite (@N_lift_dom ty) : nlift_rewrite.
+#[global] Hint Rewrite (@N_lift_dom (ty * qual)) : nlift_rewrite.
+
+Definition extends {A} (l1 l2 : list A): Prop := exists l', l1 = l' ++ l2.
+Notation "x ⊇ y" := (extends x y) (at level 0).
+
+(* Opening a term *)
+Fixpoint open_rec_tm (k : nat) (u : tm) (t : tm) {struct t} : tm :=
+  match t with
+  | tunit            => tunit
+  | tvar   (varF x) => tvar (varF x)
+  | tvar   (varB x) => if Nat.eqb k x then u else tvar (varB x)
+  | tabs    t       => tabs    (open_rec_tm (S k) u t)
+  | tapp    t1 t2   => tapp    (open_rec_tm k u t1) (open_rec_tm k u t2)
+  | tloc    l       => tloc l
+  | tref    t       => tref    (open_rec_tm k u t)
+  | tderef  t       => tderef  (open_rec_tm k u t)
+  | tassign t1 t2   => tassign (open_rec_tm k u t1) (open_rec_tm k u t2)
+  end
+.
+
+(*simultaneous opening with self-ref and argument: *)
+Definition open_tm (u t : tm) := open_rec_tm 0 u t.
+Definition open_tm' {A : Type} (env : list A) t :=
+  open_rec_tm 0 (varF (length env)) t.
+
+(* alternative without match *)
+Definition openq (u d : qual) : qual := open_qual 0 u d.
+Definition openq' {A} (env : list A) d :=
+  openq (just_fv (length env)) d.
+
+(* Opening a type with a qualifier *)
+Fixpoint open_rec_ty (k : nat) (d' : qual) (T : ty) : ty :=
+  match T with
+  | TUnit            => TUnit
+  | TFun d1 d2 T1 T2 => TFun (open_qual k d' d1) (open_qual (S k) d' d2) (open_rec_ty k d' T1) (open_rec_ty (S k) d' T2)
+  | TRef T           => TRef (open_rec_ty k d' T)
+  end.
+
+Definition open_ty (u : id) (T : ty) := (open_rec_ty 0 (just_fv u) T).
+Definition open_ty' {A : Type} (env : list A) (T : ty) :=
+  open_ty (length env) T.
+
+Module OpeningNotations.
+  Declare Scope opening.
+  Notation "[[ k ~> u ]]ᵗ t" := (open_rec_tm k u t) (at level 10) : opening.
+  Notation "[[ k ~> U ]]ᵀ T" := (open_rec_ty k U T) (at level 10) : opening.
+  Notation "[[ k ~> d' ]]ᵈ d" := (open_qual k d' d) (at level 10) : opening.
+End OpeningNotations.
+Import OpeningNotations.
+Local Open Scope opening.
+
+(* measure for induction over terms *)
+Fixpoint tm_size (t : tm) : nat :=
+  match t with
+  | tunit         => 0
+  | tvar    _     => 0
+  | tabs    t     => S (tm_size t)
+  | tapp    t1 t2 => S (tm_size t1 + tm_size t2)
+  | tloc    _     => 0
+  | tref    t     => S (tm_size t)
+  | tderef  t     => S (tm_size t)
+  | tassign t1 t2 => S (tm_size t1 + tm_size t2)
+  end.
+
+(* measure for induction over types *)
+Fixpoint ty_size (T : ty) : nat :=
+  match T with
+  | TUnit           => 0
+  | TFun  _ _ T1 T2 => S (ty_size T1 + ty_size T2)
+  | TRef  T         => S (ty_size T)
+  end.
+
+Fixpoint splice (n : nat) (t : tm) {struct t} : tm :=
+  match t with
+  | tunit          => tunit
+  | tvar (varF i)  =>
+    if le_lt_dec n i then tvar (varF (S i))
+    else tvar (varF i)
+  | tvar (varB i)  => tvar    (varB i)
+  | tabs    t      => tabs    (splice n t)
+  | tapp    t1 t2  => tapp    (splice n t1) (splice n t2)
+  | tloc    l      => tloc     l
+  | tref    t      => tref    (splice n t)
+  | tderef  t      => tderef  (splice n t)
+  | tassign t1 t2  => tassign (splice n t1) (splice n t2)
+  end.
+
+Fixpoint splice_ty (n : nat) (T : ty) {struct T} : ty :=
+  match T with
+  | TUnit            => TUnit
+  | TFun d1 d2 T1 T2 => TFun (splice_qual n d1) (splice_qual n d2) (splice_ty n T1) (splice_ty n T2)
+  | TRef T           => TRef (splice_ty n T)
+  end.
+
+Fixpoint unsplice_ty (n : nat) (T : ty) {struct T} : ty :=
+  match T with
+  | TUnit            => TUnit
+  | TFun d1 d2 T1 T2 => TFun (unsplice_qual n d1) (unsplice_qual n d2) (unsplice_ty n T1) (unsplice_ty n T2)
+  | TRef T           => TRef (unsplice_ty n T)
+  end.
+
+Fixpoint closed_tm (b f l : nat ) (t : tm) : Prop :=
+  match t with
+  | tunit          => True
+  | tvar (varF i)  => i < f
+  | tvar (varB i)  => i < b
+  | tabs    t      => closed_tm (S b) f l t
+  | tapp    t1 t2  => closed_tm b f l t1 /\ closed_tm b f l t2
+  | tloc    l'     => l' < l
+  | tref    t      => closed_tm b f l t
+  | tderef  t      => closed_tm b f l t
+  | tassign t1 t2  => closed_tm b f l t1 /\ closed_tm b f l t2
+  end.
+
+Fixpoint closed_ty (b f l : nat ) (T : ty) : Prop :=
+  match T with
+  | TUnit            => True
+  | TRef T           => closed_ty 0 0 0 T
+  | TFun d1 d2 T1 T2 =>
+      closed_Qual b f l (Q_lift d1) /\
+      closed_Qual (S b) f l (Q_lift d2) /\
+      closed_ty b f l T1 /\
+      closed_ty (S b) f l T2
+  end.
+
+Definition splice_tenv (n : nat) (Γ : tenv) : tenv :=
+  map (fun p => ((splice_ty n (fst p)), (splice_qual n (snd p)))) Γ.
+
+Inductive stp : tenv -> senv -> ty -> qual -> ty -> qual -> Prop :=
+| s_base : forall Γ Σ d1 d2,
+    Qstp (length Γ) (length Σ) (Q_lift d1) (Q_lift d2) ->
+    stp Γ Σ TUnit d1 TUnit d2
+| s_ref : forall Γ Σ T1 T2 d1 d2,
+    Qstp (length Γ) (length Σ) (Q_lift d1) (Q_lift d2) ->
+    stp [] [] T1 ∅ T2 ∅ -> (* we don't have bottom, so use ∅ here *)
+    stp [] [] T2 ∅ T1 ∅ ->
+    stp Γ Σ (TRef T1) d1 (TRef T2) d2
+| s_fun : forall Γ Σ T1 d1 T2 d2 T3 d3 T4 d4 d5 d6,
+    closed_ty 0 (length Γ) (length Σ) (TFun d1 d2 T1 T2) ->
+    closed_ty 0 (length Γ) (length Σ) (TFun d3 d4 T3 T4) ->
+    Qstp (length Γ) (length Σ) (Q_lift d5) (Q_lift d6) ->
+    stp Γ Σ T3 d3 T1 d1 ->
+    stp ((T3,d3) :: Γ) Σ (open_ty' Γ T2) (openq' Γ d2) (open_ty' Γ T4) (openq' Γ d4) ->
+    stp Γ Σ (TFun d1 d2 T1 T2) d5 (TFun d3 d4 T3 T4) d6
+| s_trans : forall Γ Σ T1 d1 T2 d2 T3 d3,
+    stp Γ Σ T1 d1 T2 d2 -> stp Γ Σ T2 d2 T3 d3 -> stp Γ Σ T1 d1 T3 d3
+.
+#[global] Hint Constructors stp : dsub.
+
+(* Specifies that the variable x's qualifier is subsumed by q in context Γ *)
+Definition saturated_var (Γ : tenv) (Σ : senv) (x : id) (q : qual)  : Prop := exists U q',
+  indexr x Γ = Some (U, q') /\
+  (Subq (Q_lift q') (Q_lift q) /\
+  closed_Qual 0 x (length Σ) (Q_lift q')).
+
+(* Specifies that q is transitively closed w.r.t. Γ, i.e., each variable x in q is a saturated variable in the above sense. *)
+Definition saturated (Γ : tenv) (Σ : senv) (q: qual) : Prop := forall x, (varF x) ∈ᵥ q -> saturated_var Γ Σ x q.
+
+(* A typing context is well-formed iff all its assumptions are saturated. *)
+Definition wf_tenv (Γ : tenv) (Σ : senv):= forall x T q, indexr x Γ = Some (T, q) -> saturated Γ Σ q.
+
+Inductive has_type : tenv -> qual -> senv -> tm -> ty -> qual -> Prop :=
+| t_base : forall Γ Σ φ,
+    closed_Qual 0 (length Γ) (length Σ) (Q_lift φ) ->
+    has_type Γ φ Σ tunit TUnit ∅ (* use ∅ instead of bottom *)
+
+| t_var : forall Γ φ Σ x T d,
+    indexr x Γ = Some (T,d) ->
+    Subq (Q_lift (d ⊕ x)) (Q_lift φ) ->
+    closed_Qual 0 (length Γ) (length Σ) (Q_lift φ) ->
+    closed_ty 0 x (length Σ) T ->
+    closed_Qual 0 x (length Σ) (Q_lift d) ->
+    has_type Γ φ Σ (tvar (varF x)) T (d ⊕ x)
+
+| t_abs: forall Γ φ Σ T1 d1 T2 d2 df t,
+    closed_tm 1 (length Γ) (length Σ) t ->
+    closed_ty 0 (length Γ) (length Σ) (TFun d1 d2 T1 T2) ->
+    closed_Qual 0 (length Γ) (length Σ) (Q_lift φ) ->
+    Subq (Q_lift df) (Q_lift φ) ->
+    saturated Γ Σ d1 ->
+    saturated Γ Σ df ->
+    has_type ((T1,d1) :: Γ) (df ⊔ (just_fv (length Γ))) Σ (open_tm' Γ t) (open_ty' Γ T2) (openq' Γ d2) ->
+    has_type Γ φ Σ (tabs t) (TFun d1 d2 T1 T2) df
+
+| t_app : forall Γ φ Σ t1 d1 t2 d2 df T1 T2,
+    has_type Γ φ Σ t1 (TFun (df ⊓ d1) d2 T1 T2) df ->
+    has_type Γ φ Σ t2 T1 d1 ->
+    closed_ty 0 (length Γ) (length Σ) T2 ->
+    Subq (Q_lift (openq ∅ d2)) (Q_lift φ) ->
+    saturated Γ Σ (openq ∅ d2) ->
+    has_type Γ φ Σ (tapp t1 t2) T2 (openq d1 d2)
+
+| t_loc : forall Γ φ Σ l T,
+    closed_Qual 0 (length Γ) (length Σ) (Q_lift φ) ->
+    indexr l Σ = Some T ->
+    closed_ty 0 0 0 T ->
+    Subq (Q_lift (just_loc l)) (Q_lift φ) ->
+    has_type Γ φ Σ (tloc l) (TRef T) (just_loc l)
+
+| t_ref: forall Γ φ Σ t d,
+    has_type Γ φ Σ t TUnit d   ->
+    has_type Γ φ Σ (tref t) (TRef TUnit) ∅
+
+| t_deref: forall Γ φ Σ T d t,
+    has_type Γ φ Σ t (TRef T) d ->
+    has_type Γ φ Σ (tderef t) T ∅
+
+| t_assign: forall Γ φ Σ t1 t2 d1 d2,
+    has_type Γ φ Σ t1 (TRef TUnit) d1 ->
+    has_type Γ φ Σ t2 TUnit d2 ->
+    has_type Γ φ Σ (tassign t1 t2) TUnit ∅
+
+| t_sub: forall Γ φ  Σ e T1 d1 T2 d2,
+    has_type Γ φ Σ e T1 d1 ->
+    stp Γ Σ T1 d1 T2 d2 ->
+    Subq (Q_lift d2) (Q_lift φ) ->
+    saturated Γ Σ d2 ->
+    has_type Γ φ Σ e T2 d2
+.
+#[global] Hint Constructors has_type : core.
+
+Inductive value : tm -> Prop :=
+| value_abs : forall t, value (tabs t)
+| value_cst : value tunit
+| value_loc : forall l, value (tloc l)
+.
+#[global] Hint Constructors value : core.
+
+Definition store := list tm.
+
+Inductive step : tm -> store -> tm -> store -> Prop :=
+(*contraction rules*)
+| step_beta : forall t v σ,
+    value v ->
+    step (tapp (tabs t) v) σ (open_tm v t) σ
+| step_ref : forall v σ,
+    value v ->
+    step (tref v) σ (tloc (length σ)) (v :: σ)
+| step_deref : forall σ l v,
+    indexr l σ = Some v ->
+    step (tderef (tloc l)) σ v σ
+| step_assign : forall σ l v,
+    l < (length σ) ->
+    value v ->
+    step (tassign (tloc l) v) σ tunit (update σ l v)
+(*congruence rules*)
+| step_c_ref : forall t t' σ σ',
+    step t σ t' σ' ->
+    step (tref t) σ (tref t') σ'
+| step_c_deref : forall t t' σ σ',
+    step t σ t' σ' ->
+    step (tderef t) σ (tderef t') σ'
+| step_c_app_l : forall t1 t1' t2 σ σ',
+    step t1 σ t1' σ' ->
+    step (tapp t1 t2) σ (tapp t1' t2) σ'
+| step_c_app_r : forall v t2 t2' σ σ',
+    value v ->
+    step t2 σ t2' σ' ->
+    step (tapp v t2) σ (tapp v t2') σ'
+| step_c_assign_l : forall t1 t1' t2 σ σ',
+    step t1 σ t1' σ' ->
+    step (tassign t1 t2) σ (tassign t1' t2) σ'
+| step_c_assign_r : forall v t2 t2' σ σ',
+    value v ->
+    step t2 σ t2' σ' ->
+    step (tassign v t2) σ (tassign v t2') σ'
+.
+
+Definition CtxOK (Γ : tenv) (φ : qual) (Σ : senv) (σ : store) : Prop :=
+  length Σ = length σ /\
+  forall l v T, indexr l Σ = Some T -> indexr l σ = Some v -> value v /\ has_type Γ φ Σ v T ∅.
+
+(* Substitutions
+
+   It is assumed that substitution is always on the first two context entries, which
+   is why other free variables are unconditionally decremented.
+*)
+Fixpoint subst_tm (t : tm) (v : nat) (u : tm) : tm :=
+  match t with
+  | tunit         => tunit
+  | # x           => # x
+  | $ x           => if Nat.eqb x v then u else $(pred x)
+  | tabs t        => tabs (subst_tm t v u)
+  | tapp t1 t2    => tapp (subst_tm t1 v u) (subst_tm t2 v u)
+  | & l           => & l
+  | tref t        => tref (subst_tm t v u)
+  | ! t           => ! (subst_tm t v u)
+  | tassign t1 t2 => tassign (subst_tm t1 v u) (subst_tm t2 v u)
+  end.
+Notation "{ v1 |-> t1 ; t2 }ᵗ t" := (subst_tm (subst_tm t v1 t1) v1 t2) (at level 10).
+Notation "{ v1 |-> t1 }ᵗ t" := (subst_tm t v1 t1) (at level 10).
+
+Fixpoint subst_ty (T : ty) (v : nat) (q : qual) : ty :=
+  match T with
+  | TUnit            => TUnit
+  | TFun q1 q2 T1 T2 => TFun (subst_qual q1 v q) (subst_qual q2 v q) (subst_ty T1 v q) (subst_ty T2 v q)
+  | TRef T           => TRef (subst_ty T v q)
+  end.
+
+Definition subst_tenv (Γ : tenv) (v : nat) (q1 : qual) : tenv :=
+  map (fun p => match p with
+             | (T,q') => ((subst_ty T v q1) , (subst_qual q' v q1))
+             end) Γ.
+
+Module SubstitutionNotations.
+  Declare Scope substitutions.
+  Notation "{ v1 |-> t1 ; t2 }ᵗ t" := (subst_tm (subst_tm t v1 t1) v1 t2) (at level 10) : substitutions.
+  Notation "{ v1 |-> t1 }ᵗ t" := (subst_tm t v1 t1) (at level 10) : substitutions.
+  Notation "{ v1 |-> q1 ; q2 }ᵈ q" := (subst_qual (subst_qual q v1 q1) v1 q2) (at level 10) : substitutions.
+  Notation "{ v1 |-> q1 }ᵈ q" := (subst_qual q v1 q1) (at level 10) : substitutions.
+  Notation "{ v1 |-> q1 ; q2  }ᵀ T" := (subst_ty (subst_ty T v1 q1) v1 q2) (at level 10) : substitutions.
+  Notation "{ v1 |-> q1 }ᵀ T" := (subst_ty T v1 q1) (at level 10) : substitutions.
+  Notation "{ v1 |-> q1 }ᴳ G" := (subst_tenv G v1 q1) (at level 10) : substitutions.
+  Notation "{ v1 |-> q1 ; q2 }ᴳ G" := (subst_tenv (subst_tenv G v1 q1) v1 q2) (at level 10) : substitutions.
+End SubstitutionNotations.
+Import SubstitutionNotations.
+Local Open Scope substitutions.
+
+(* Indicates that d is freshly picked w.r.t to the store typing Σ and contained in Σ'.
+   This is used in the type safety theorem to specify that steps may only introduce a fresh qualifier from storage effects.
+   More specifically, the "fresh" qualifier d is at most a singleton containing a fresh store location. *)
+Inductive disjointq (Σ Σ' : senv) (d : qual) : Prop :=
+| disj_bot : d = ∅ -> disjointq Σ Σ' d
+| disj_loc : forall l,
+    (length Σ) <= l ->
+    l < (length Σ') ->
+    d = (just_loc l) -> disjointq Σ Σ' d
+.
+Arguments disj_loc { Σ Σ' d }.
+#[global] Hint Constructors disjointq : core.
+
+(* :! -- directly invertible value typing *)
+
+Inductive vtp: senv -> tm -> ty -> qual -> Prop :=
+| vtp_base: forall Σ d,
+  closed_Qual 0 0 (length Σ) (Q_lift d) ->
+  vtp Σ tunit TUnit d
+
+| vtp_loc:  forall Σ l T U d,
+  closed_Qual 0 0 (length Σ) (Q_lift d) ->
+  closed_ty 0 0 0 T ->
+  indexr l Σ = Some T ->
+  stp [] [] T ∅ U ∅ -> (* we don't have bottom, so use ∅ here *)
+  stp [] [] U ∅ T ∅ ->
+  Qstp 0 (length Σ) (Q_lift (just_loc l)) (Q_lift d) ->
+  vtp Σ (tloc l) (TRef U) d
+
+| vtp_abs: forall Σ T1 d1 T2 d2 T3 d3 T4 d4 df1 df2 t,
+  closed_tm 1 0 (length Σ) t ->
+  closed_Qual 0 0 (length Σ) (Q_lift df2) ->
+  closed_ty 0 0 (length Σ) (TFun d3 d4 T3 T4) ->  (* sub type *)
+  closed_ty 0 0 (length Σ) (TFun d1 d2 T1 T2) ->  (* super type *)
+  has_type [(T1,d1)] (df1 ⊔ (just_fv 0)) Σ (open_tm' ([]: tenv) t) (open_ty' ([]: tenv) T2) (openq' ([]: tenv) d2) ->
+  stp [] Σ T3 d3 T1 d1 ->
+  Qstp 0 (length Σ) (Q_lift df1) (Q_lift df2) ->
+  stp [(T3, d3)] Σ (open_ty' ([]: tenv) T2) (openq' ([] : tenv) d2) (open_ty' ([]: tenv) T4) (openq' ([]: tenv) d4) ->
+  vtp Σ (tabs t) (TFun d3 d4 T3 T4) df2
+  .
+#[global] Hint Constructors vtp : core.
+
+(* The concluding statement of the preservation part of type safety, i.e., typing is preserved after a step under an extended store, so
+   that the initial qualifier is increased by at most a fresh storage effect. *)
+Inductive preserve (Γ : tenv) (Σ : senv) (t' : tm) (T : ty) (d : qual) (σ' : store) : Prop :=
+| Preserve : forall Σ' d',
+    Σ' ⊇ Σ ->
+    CtxOK Γ (qdom Σ') Σ' σ' ->
+    disjointq Σ Σ' d' ->
+    has_type Γ (qdom Σ') Σ' t' T (d ⊔ d') ->
+    preserve Γ Σ t' T d σ'.
+Arguments Preserve {Γ Σ t' T d σ'}.
+
+(* deterministic relations (used to recover standard progress & preservation from the type safety theorem. ) *)
+Definition relation (X : Type)(Y: Type) := X -> Y -> X ->  Y -> Prop.
+Definition deterministic {X : Type}{Y: Type} (R : relation X Y) :=
+  forall (x x1 x2 : X) (y y1 y2: Y), R x y x1 y1 -> R x y x2 y2 -> x1 = x2 /\ y1 = y2.
+
+(* The concluding statement of the separation of preservation corollary, i.e., interleaving the execution of two well-typed
+   terms with disjoint qualifiers preserves the types and keeps qualifiers disjoint.  *)
+Inductive separate (Σ : senv) (t1' : tm) (T1 : ty) (t2' : tm) (T2 : ty) : Prop :=
+| Separate : forall Σ' Σ'' q1' q2',
+    Σ' ⊇ Σ ->
+    Σ'' ⊇ Σ' ->
+    has_type [] (qdom Σ') Σ' t1' T1 q1' ->
+    has_type [] (qdom Σ'') Σ'' t2' T2 q2' ->
+    q1' ⊓ q2' ⊑↑ ∅ ->
+    separate Σ t1' T1 t2' T2.
+Arguments Separate {Σ t1' T1 t2' T2}.
+
+(** Metatheory **)
+
+Lemma extends_refl : forall {A}, forall{l : list A}, extends l l.
+  intros. unfold extends. exists []. auto.
+Qed.
+#[global] Hint Resolve extends_refl : core.
+
+Lemma extends_cons : forall {A}, forall{l : list A}, forall{a:A}, extends (a :: l) l.
+  intros. unfold extends. exists [a]. auto.
+Qed.
+
+Lemma extends_length : forall {A}, forall{l1 l2 : list A}, extends l1 l2 -> length l1 >= length l2.
+  intros. unfold extends in H. destruct H as [l' Heq]. subst. rewrite app_length. lia.
+Qed.
+
+Lemma extends_ldom : forall {Σ' Σ : senv}, (Σ') ⊇ (Σ) -> qdom Σ ⊑↑ qdom Σ'.
+  intros. inversion H. unfold qdom. simpl.
+  intuition. assert (length Σ' = length (x ++ Σ)). subst. auto.
+  rewrite app_length in H1. assert (length Σ <= length Σ'). lia.
+  unfold Subq. unfold_N. intuition. simpl in *. apply Nat.ltb_lt in H3. apply Nat.ltb_lt. lia.
+Qed.
+
+Lemma open_tm'_len : forall {A} {Γ Γ' : list A} {t}, length Γ = length Γ' -> open_tm' Γ t = open_tm' Γ' t.
+  intros.  unfold open_tm'. rewrite H. auto.
+Qed.
+
+Lemma open_ty'_len : forall {A} {Γ Γ' : list A} {T}, length Γ = length Γ' -> open_ty' Γ T = open_ty' Γ' T.
+  intros.  unfold open_ty'. rewrite H. auto.
+Qed.
+
+Lemma openq'_len : forall {A} {Γ Γ' : list A} {q}, length Γ = length Γ' -> openq' Γ q = openq' Γ' q.
+  intros.  unfold openq'. rewrite H. auto.
+Qed.
+
+Lemma open_preserves_size: forall t x j, tm_size t = tm_size (open_rec_tm j (tvar x) t).
+  induction t; intros; simpl; eauto.
+  destruct v. auto. destruct (Nat.eqb j i); auto.
+Qed.
+
+Lemma open_ty_preserves_size: forall T d j, ty_size T = ty_size (open_rec_ty j d T).
+  induction T; intros; simpl; eauto.
+Qed.
+
+Lemma splice_qual_empty : forall {k}, splice_qual k ∅ = ∅.
+  intros. simpl. unfold_q. repeat f_equal.
+  apply N_lift_eq. nlift. unfold_N. intuition.
+Qed.
+#[global] Hint Resolve splice_qual_empty : core.
+
+Lemma closed_qual_ldom : forall {Σ : senv}, closed_Qual 0 0 (length Σ) (Qdom Σ).
+  intros. unfold_Q; unfold_N; unfold N_lift; intuition.
+Qed.
+#[global] Hint Resolve closed_qual_ldom : core.
+
+(* This property is specific to the restricted version of the system we consider here *)
+Lemma qstp_inv : forall {Γ Σ d1 d2}, qstp Γ Σ d1 d2 -> d1 ⊑↑ d2.
+  intros. inversion H. auto.
+Qed.
+
+Lemma splice_tenv_length : forall {n Γ}, length (splice_tenv n Γ) = length Γ.
+  intros. unfold splice_tenv. rewrite map_length. auto.
+Qed.
+
+Lemma closed_tm_monotone : forall {t b l f}, closed_tm b f l t -> forall {b' f' l'}, b <= b' -> f <= f' -> l <= l' -> closed_tm b' f' l' t.
+intros T. induction T; simpl in *; intuition; eauto. destruct v; intuition. eapply IHT; eauto. lia.
+Qed.
+
+Lemma closed_ty_monotone : forall {T b l f}, closed_ty b f l T -> forall {b' f' l'}, b <= b' -> f <= f' -> l <= l' -> closed_ty b' f' l' T.
+Proof.
+  intros T b l f H. generalize dependent b. induction T; unfold_Q; intuition eauto 3 with arith.
+Qed.
+#[global] Hint Resolve closed_ty_monotone : core.
+
+Lemma closed_tm_open_id : forall {t b f l}, closed_tm b f l t -> forall {n}, b <= n -> forall {x}, (open_rec_tm n x t) = t.
+intros t b f l H. generalize dependent b. induction t; intros; simpl in *; intuition;
+    try solve [erewrite IHt1; eauto; erewrite IHt2; eauto; lia | erewrite IHt; eauto; lia].
+  destruct v eqn:Eqv; auto. bdestruct (n =? i); auto. lia.
+Qed.
+
+Lemma closed_ty_open_id : forall {t b f l}, closed_ty b f l t -> forall {n}, b <= n -> forall {x}, (open_rec_ty n x t) = t.
+intros t b f l H. generalize dependent b. induction t; intros; simpl in *; intuition.
+erewrite IHt1; eauto; erewrite IHt2; eauto. repeat erewrite closed_qual_open_id; eauto. lia. lia.
+  erewrite IHt; eauto. eapply closed_ty_monotone; eauto; lia.
+Qed.
+
+Lemma closed_tm_open' : forall {T b f l}, closed_tm (S b) f l T -> forall {x}, x <= f -> forall {t}, closed_tm 0 x l t -> closed_tm b f l (open_rec_tm b t T).
+induction T; intros; simpl in *; intuition;
+  try solve [eapply IHT1; eauto | eapply IHT2; eauto | eapply IHT; eauto ].
+  destruct v; auto. bdestruct (b =? i); subst. eapply closed_tm_monotone; eauto; lia.
+  simpl. lia.
+Qed.
+
+Lemma closed_ty_open' : forall {T b f l}, closed_ty (S b) f l T -> forall {x}, x <= f -> forall {d}, closed_Qual 0 x l (Q_lift d) -> closed_ty b f l (open_rec_ty b d T).
+  induction T; intros; simpl in *; intuition.
+  1,2 : rewrite Q_lift_open_qual; eapply closed_qual_open'; eauto.
+  all: try solve [eapply IHT1; eauto | eapply IHT2; eauto | eapply IHT; eauto ].
+  erewrite closed_ty_open_id; eauto. lia.
+Qed.
+
+Lemma splice_tm_id : forall {T b f l}, closed_tm b f l T -> (splice f T ) = T.
+induction T; intros; simpl in *; auto; intuition;
+    try solve [erewrite IHT1; eauto; erewrite IHT2; eauto | erewrite IHT; eauto].
+    destruct v; auto. destruct (le_lt_dec f i) eqn:Heq. lia. auto.
+Qed.
+
+Lemma splice_ty_id : forall {T b f l},
+  closed_ty b f l T ->
+  (splice_ty f T) = T.
+induction T; intros; simpl in *; auto; f_equal; intuition eauto using splice_qual_id.
+eapply IHT; eapply closed_ty_monotone; eauto; lia.
+Qed.
+
+Lemma splice_tm_open : forall {T j n m}, splice n (open_rec_tm j (varF (m + n)) T) = open_rec_tm j (varF (S (m + n))) (splice n T).
+  induction T; intros; simpl; auto;
+    try solve [erewrite IHT1; eauto; erewrite IHT2; eauto | erewrite IHT; eauto].
+  destruct v; simpl. destruct (le_lt_dec n i) eqn:Heq; auto.
+  destruct (PeanoNat.Nat.eqb j i) eqn:Heq; auto.
+  simpl. destruct (le_lt_dec n (m + n)) eqn:Heq'. auto. lia.
+Qed.
+
+Lemma splice_ty_open : forall {T j n m}, splice_ty n (open_rec_ty j (just_fv (m + n)) T) = open_rec_ty j (just_fv (S (m + n))) (splice_ty n T).
+  induction T; intros; simpl; auto;
+    try solve [erewrite IHT1; eauto; erewrite IHT2; eauto | erewrite IHT; eauto]. rewrite splice_qual_open. rewrite splice_qual_open. rewrite IHT1. rewrite IHT2. auto.
+Qed.
+
+Lemma splice_tm_open' : forall {T} {A} {D : A} {ρ ρ'}, splice (length ρ') (open_tm' (ρ ++ ρ') T) = open_tm' (ρ ++ D :: ρ') (splice (length ρ') T).
+  intros. unfold open_tm'.
+  replace (length (ρ ++ ρ')) with ((length ρ) + (length ρ')).
+  replace (S (length (ρ ++ D :: ρ'))) with (S (S (length ρ) + (length ρ'))).
+  replace (length (ρ ++ D :: ρ')) with (S ((length ρ) + (length ρ'))).
+  rewrite <- splice_tm_open. auto.
+  all: rewrite app_length; simpl; lia.
+Qed.
+
+Lemma splice_qual_open' : forall {d} {A} {D : A} {ρ ρ'}, splice_qual (length ρ') (openq' (ρ ++ ρ') d) = openq' (ρ ++ D :: ρ') (splice_qual (length ρ') d).
+  intros. unfold openq'. unfold openq.
+  replace (length (ρ ++ ρ')) with ((length ρ) + (length ρ')).
+  replace (S (length (ρ ++ D :: ρ'))) with (S (S (length ρ) + (length ρ'))).
+  replace (length (ρ ++ D :: ρ')) with (S ((length ρ) + (length ρ'))).
+  rewrite <- splice_qual_open. auto.
+  all: rewrite app_length; simpl; lia.
+Qed.
+
+Lemma splice_ty_open' : forall {T} {A} {D : A} {ρ ρ'}, splice_ty (length ρ') (open_ty' (ρ ++ ρ') T) = open_ty' (ρ ++ D :: ρ') (splice_ty (length ρ') T).
+  intros. unfold open_ty'. unfold open_ty.
+  replace (length (ρ ++ ρ')) with ((length ρ) + (length ρ')).
+  replace (S (length (ρ ++ D :: ρ'))) with (S (S (length ρ) + (length ρ'))).
+  replace (length (ρ ++ D :: ρ')) with (S ((length ρ) + (length ρ'))).
+  rewrite <- splice_ty_open. auto.
+  all: rewrite app_length; simpl; lia.
+Qed.
+
+Lemma splice_tm_closed : forall {T b n m l}, closed_tm b (n + m) l T -> closed_tm b (S (n + m)) l (splice m T).
+  induction T; simpl; intros; intuition.
+  destruct v; intuition.
+  destruct (le_lt_dec m i) eqn:Heq; simpl; lia.
+Qed.
+
+Lemma splice_Qual_closed : forall {d b n m l},
+    closed_Qual b (n + m)     l d ->
+    forall {i}, i <= m -> closed_Qual b (S (n + m)) l (splice_Qual i d).
+Proof.
+  intros. qual_destruct d. unfold_Q. intuition.
+Qed.
+
+Lemma splice_ty_closed : forall {T b n m l}, closed_ty b (n + m) l T -> forall {i}, i <= m -> closed_ty b (S (n + m)) l (splice_ty i T).
+  induction T; simpl; intros; intuition.
+  1,2 : rewrite Q_lift_splice_qual; apply splice_Qual_closed; auto.
+  erewrite splice_ty_id; eauto. eapply closed_ty_monotone; eauto. lia.
+Qed.
+
+Lemma splice_closed' : forall {T b l} {A} {D : A} {ρ ρ'},
+    closed_tm b (length (ρ ++ ρ')) l T ->  closed_tm b (length (ρ ++ D :: ρ')) l (splice (length ρ') T).
+  intros. rewrite app_length in H.
+  replace (length (ρ ++ D :: ρ')) with (S (length ρ) + (length ρ')).
+  apply splice_tm_closed. auto. simpl. rewrite app_length. simpl. lia.
+Qed.
+
+Lemma splice_qual_closed' : forall {d b l} {A} {D : A} {ρ ρ'},
+    closed_Qual b (length (ρ ++ ρ')) l d -> closed_Qual b (length (ρ ++ D :: ρ')) l (splice_Qual (length ρ') d).
+  intros. rewrite app_length in H.
+  replace (length (ρ ++ D :: ρ')) with (S (length ρ) + (length ρ')).
+  eapply splice_Qual_closed; eauto. simpl. rewrite app_length. simpl. lia.
+Qed.
+
+Lemma splice_ty_closed' : forall {T b l} {A} {D : A} {ρ ρ'},
+    closed_ty b (length (ρ ++ ρ')) l T -> closed_ty b (length (ρ ++ D :: ρ')) l (splice_ty (length ρ') T).
+  intros. rewrite app_length in H.
+  replace (length (ρ ++ D :: ρ')) with (S (length ρ) + (length ρ')).
+  eapply splice_ty_closed; eauto. simpl. rewrite app_length. simpl. lia.
+Qed.
+
+Lemma splice_ty_closed'' : forall {T x b l k}, closed_ty b x l T -> k <= x -> closed_ty b (S x) l (splice_ty k T).
+  induction T; simpl; intros; intuition.
+  1,2: rewrite Q_lift_splice_qual; unfold_Q; intuition.
+  erewrite splice_ty_id; eauto.
+  eapply closed_ty_monotone; eauto. lia.
+Qed.
+
+Lemma splice_qual_open'' : forall {k df d},
+    splice_qual k (openq df d) =
+    openq (splice_qual k df) (splice_qual k d).
+Proof.
+  intros. qual_destruct d; qual_destruct df; simpl.
+  unfold openq. unfold_q. destruct (bvs 0); auto.
+  unfold_n. repeat f_equal. apply functional_extensionality. intros.
+  bdestruct (x =? k); bdestruct (x <? k); intuition.
+Qed.
+
+Lemma splice_qual_qplus_dist : forall {i k d},
+    k <= i -> (splice_qual k d ⊕ S i) = splice_qual k (d ⊕ i).
+Proof.
+  intros. qual_destruct d. simpl. unfold_q. unfold_n. repeat f_equal. apply functional_extensionality. intuition. bdestruct (x =? k). subst. simpl. apply Nat.eqb_neq. lia. bdestruct (x <? k). destruct (fvs x); auto. bdestruct (x =? i); bdestruct (x =? S i); intuition.
+  destruct (fvs (Init.Nat.pred x)); auto. bdestruct ((x =? S i)); bdestruct (Init.Nat.pred x =? i); intuition.
+Qed.
+
+Lemma splice_Qual_qplus_id : forall {i k l d},
+    closed_Qual 0 i l (Q_lift d) -> i < k -> splice_Qual k (Q_lift (d ⊕ i)) = (Q_lift (d ⊕ i)).
+Proof.
+  intros. qual_destruct d. unfold_Q. unfold_q. repeat rewrite N_lift_or. repeat rewrite N_lift_one. repeat rewrite N_lift_empty. repeat f_equal. unfold_N. apply functional_extensionality. intros. apply propositional_extensionality. intuition.
+  - bdestruct (x =? i). right. auto. left. bdestruct (x <? k); intuition. assert (x > k) by lia. intuition. apply H1 in H6. lia.
+  - subst. apply H1 in H4. lia.
+  - destruct (fvs (Init.Nat.pred x)) eqn:Eqm. left. unfold N_lift. auto. right. apply H1 in H4. lia.
+Qed.
+
+Lemma splice_qual_qplus_id : forall {i k l d},
+    closed_Qual 0 i l (Q_lift d) -> i < k -> splice_qual k (d ⊕ i) = (d ⊕ i).
+Proof.
+  intros. pose proof (splice_Qual_qplus_id H H0). unfold_Q. unfold_N. qual_destruct d. unfold Q_lift,N_lift in *. unfold_q. unfold_n. repeat f_equal. apply functional_extensionality. intuition. bdestruct (x=?k).
+  - subst. bdestruct (k =? i); intuition. destruct (fvs k) eqn:Eq; intuition. apply H2 in Eq. lia.
+  - bdestruct (x <? k); intuition. destruct (fvs x) eqn:Eq1;destruct (fvs (Init.Nat.pred x)) eqn:Eq2; bdestruct (x =? i); bdestruct (Init.Nat.pred x =? i); intuition. apply H2 in Eq1. lia.  apply H2 in Eq2. lia.
+Qed.
+
+Lemma qplus_closed_qual : forall {d b f l x},
+    closed_Qual b f l (Q_lift d) ->
+    forall {f'}, f <= f' -> x < f' -> closed_Qual b f' l (Q_lift (d ⊕ x)).
+Proof.
+  intros. qual_destruct d. rewrite Q_lift_or. unfold_Q. unfold_q. rewrite N_lift_one. rewrite N_lift_empty. unfold_N. intuition eauto using Nat.lt_le_trans. rewrite H5. auto.
+Qed.
+#[global] Hint Resolve qplus_closed_qual : core.
+
+Lemma stp_closed : forall {Γ Σ T1 d1 T2 d2},
+    stp Γ Σ T1 d1 T2 d2 ->
+    closed_ty 0 (length Γ) (length Σ) T1
+    /\ closed_Qual 0 (length Γ) (length Σ) (Q_lift d1)
+    /\ closed_ty 0 (length Γ) (length Σ) T2
+    /\ closed_Qual 0 (length Γ) (length Σ) (Q_lift d2).
+Proof.  intros Γ Σ T1 d1 T2 d2 HS. induction HS. 1,2: qual_destruct d1; qual_destruct d2; unfold_Q; unfold_N; intuition eauto.
+- qual_destruct d5. qual_destruct d6. unfold_Q. unfold_N. intuition eauto.
+- intuition.
+Qed.
+
+Lemma stp_refl : forall {n T}, ty_size T < n -> forall {Γ Σ}, closed_ty 0 (length Γ) (length Σ) T -> forall {d d'}, Qstp (length Γ) (length Σ) (Q_lift d) (Q_lift d') -> stp Γ Σ T d T d'.
+  induction n; try lia; destruct T; simpl; intros Hsize Γ Σ Hc d d' Hstp; intuition.
+  - (*TFun*) constructor; simpl; auto. apply IHn. lia. auto. apply Qstp_refl; auto. apply IHn. unfold open_ty'. unfold open_ty. rewrite <- open_ty_preserves_size. lia. simpl. unfold open_ty'. unfold open_ty.
+    eapply closed_ty_open' with (x:=S (length Γ)); eauto. unfold_Q. nlift. unfold_N. intuition. unfold openq',openq. rewrite Q_lift_open_qual. constructor. unfold_Q. nlift. unfold_N. intuition.
+    unfold_Q. nlift. unfold_N.
+    ndestruct (snd (fst q0) 0); intuition. eapply closed_Nats_tighten; eauto.
+  - (*TRef*) constructor. auto.
+    all : apply IHn; try lia; auto. all: unfold_Q; nlift; unfold_N; intuition.
+Qed.
+
+Lemma stp_refl_qual : forall {Γ Σ T0 d0 T1 d1 d2},
+  stp Γ Σ T0 d0 T1 d1 ->
+  closed_Qual 0 (length Γ) (length Σ) (Q_lift d2) ->
+  stp Γ Σ T0 d2 T1 d2.
+intros. induction H.
+  - eapply stp_refl; eauto. constructor. Qcrush.
+  - constructor; auto. Qcrush.
+  - constructor; auto. Qcrush.
+  - apply s_trans with (d2:=d2) (T2:=T2).
+    apply IHstp1. Qcrush.
+    apply IHstp2. Qcrush.
+Qed.
+
+Lemma stp_qstp_inv : forall {Γ Σ T1 d1 T2 d2}, stp Γ Σ T1 d1 T2 d2 -> Qstp (length Γ) (length Σ) (Q_lift d1) (Q_lift d2).
+  intros Γ Σ T1 d1 T2 d2 HS. induction HS; intuition. eapply qstp_trans; eauto.
+Qed.
+
+Lemma weaken_qstp_gen : forall {Γ1 Γ2 Σ d1 d2},
+    Qstp (length (Γ1 ++ Γ2)) Σ d1 d2 ->
+    forall T', Qstp (length ((splice_tenv (length Γ2) Γ1) ++ T' :: Γ2)) Σ (splice_Qual (length Γ2) d1) (splice_Qual (length Γ2) d2).
+Proof.
+  intros Γ1 Γ2 Σ d1 d2 HSTP (T', d'). inversion HSTP. subst.
+  qual_destruct d1. qual_destruct d2.
+  constructor; unfold_Q; intuition.
+  rewrite app_length in *. rewrite splice_tenv_length. simpl. rewrite <- plus_n_Sm. intuition.
+Qed.
+
+Lemma weaken_stp_gen : forall {Γ1 Γ2 Σ T1 d1 T2 d2},  stp (Γ1 ++ Γ2) Σ T1 d1 T2 d2 ->
+    forall T', stp ((splice_tenv (length Γ2) Γ1) ++ T' :: Γ2) Σ (splice_ty (length Γ2) T1) (splice_qual (length Γ2) d1) (splice_ty (length Γ2) T2) (splice_qual (length Γ2) d2).
+Proof. intros Γ1 Γ2 Σ T1 d1 T2 d2  Hstp T'. remember (Γ1 ++ Γ2)  as Γ. generalize dependent Γ1. induction Hstp; intros.
+- subst. constructor. qual_destruct d1. qual_destruct d2. unfold_Q. unfold_q. repeat rewrite N_lift_splice. rewrite app_length in *. rewrite splice_tenv_length. simpl. rewrite <- plus_n_Sm. intuition eauto.
+  - assert (stp Γ Σ (TRef T1) d1 (TRef T2) d2). { constructor; intuition. } subst.
+    apply stp_closed in H0 as Hcl. intuition. simpl in *.
+    replace (splice_ty (length Γ2) T1) with T1. replace (splice_ty (length Γ2) T2) with T2.
+    constructor; auto; fold splice_ty.
+    qual_destruct d1. qual_destruct d2. unfold_Q. unfold_q. repeat rewrite N_lift_splice. rewrite app_length in *. rewrite splice_tenv_length. simpl. rewrite <- plus_n_Sm. simpl. intuition eauto.
+    1,2 : erewrite splice_ty_id; eauto; eapply closed_ty_monotone; eauto; lia.
+  - assert (stp Γ Σ (TFun d1 d2 T1 T2) d5 (TFun d3 d4 T3 T4) d6). { constructor; intuition. } intros.
+    subst. simpl in *. apply qstp_closed in H1 as Hcl. intuition.
+    qual_destruct d1. qual_destruct d2. qual_destruct d3. qual_destruct d4. qual_destruct d5. qual_destruct d6.
+    constructor; try fold splice_ty.
+    1-3: rewrite app_length in *; rewrite splice_tenv_length in *; simpl; rewrite <- plus_n_Sm; unfold_Q; unfold_q; repeat rewrite N_lift_splice in *; intuition eauto using splice_ty_closed.
+    specialize (IHHstp1 Γ1). intuition.
+    specialize (IHHstp2 ((T3, (fvs1, bvs1, lcs1)) :: Γ1)). intuition.
+    repeat rewrite <- splice_ty_open'. repeat rewrite <- splice_qual_open'. unfold open_ty' in *. unfold open_ty in *. unfold openq' in *. unfold openq in *. rewrite app_length in *. rewrite splice_tenv_length. simpl. auto.
+  - intros. specialize (IHHstp1 Γ1). specialize (IHHstp2 Γ1). intuition.
+    eapply s_trans; eauto.
+Qed.
+
+Lemma weaken_stp : forall {Γ Σ T1 d1 T2 d2}, stp Γ Σ T1 d1 T2 d2 -> forall T', stp (T' :: Γ) Σ T1 d1 T2 d2.
+Proof. intros Γ Σ T1 d1 T2 d2 HST. specialize (@weaken_stp_gen [] Γ Σ T1 d1 T2 d2) as Hsp. simpl in *.  specialize (Hsp HST).
+       intros.  specialize (Hsp T'). apply stp_closed in HST. intuition. replace (splice_ty (length Γ) T1) with T1 in Hsp.
+       replace (splice_ty (length Γ) T2) with T2 in Hsp.
+       replace (splice_qual (length Γ) d1) with d1 in Hsp.
+       replace (splice_qual (length Γ) d2) with d2 in Hsp. intuition.
+       1,2 : erewrite  splice_qual_id; eauto.
+       1,2 : erewrite splice_ty_id; eauto.
+Qed.
+
+Lemma weaken_stp' : forall {Γ Σ T1 d1 T2 d2}, stp Γ Σ T1 d1 T2 d2 -> forall Γ', stp (Γ' ++ Γ) Σ T1 d1 T2 d2.
+  intros. induction Γ'.
+  - simpl. auto.
+  - replace ((a :: Γ') ++ Γ) with (a :: (Γ' ++ Γ)).
+    apply weaken_stp. auto. simpl. auto.
+Qed.
+Lemma weaken_stp_store : forall {Σ Γ T1 d1 T2 d2}, stp Γ Σ T1 d1 T2 d2 -> forall Σ', stp Γ (Σ' ++ Σ) T1 d1 T2 d2.
+Proof.
+  intros Σ Γ T1 d1 T2 d2 HSTP. induction HSTP; intros.
+  1-3: constructor; auto; unfold_Q; rewrite app_length; intuition eauto using closed_Nats_mono,le_plus_r.
+  specialize (IHHSTP1 Σ'). specialize (IHHSTP2 Σ'). eapply s_trans in IHHSTP2; eauto.
+Qed.
+
+Lemma weaken_stp_store_ext : forall {Σ Γ T1 d1 T2 d2}, stp Γ Σ T1 d1 T2 d2 -> forall {Σ'}, Σ' ⊇ Σ ->  stp Γ Σ' T1 d1 T2 d2.
+  intros. unfold extends in H0. destruct H0. subst. apply weaken_stp_store. auto.
+Qed.
+
+Lemma narrowing_Qstp_gen : forall{Γ1 U du Γ2 Σ d1 d2},
+    Qstp (length (Γ1 ++ (U,du) :: Γ2)) (length Σ) d1 d2 ->
+    forall {V dv}, stp Γ2 Σ V dv U du ->
+              Qstp (length (Γ1 ++ (V,dv) :: Γ2)) (length Σ) d1 d2.
+  intros Γ1 U du Γ2 Σ d1 d2 HQ V dv HSTP.
+  inversion HQ. subst. constructor.
+  auto. rewrite app_length in *. simpl in *. auto.
+Qed.
+
+Lemma narrowing_stp_gen : forall{Γ1 U du Γ2 Σ T1 d1 T2 d2}, stp (Γ1 ++ (U,du) :: Γ2) Σ T1 d1 T2 d2 -> forall {V dv}, (stp Γ2 Σ V dv U du) -> stp (Γ1 ++ (V,dv) :: Γ2) Σ T1 d1 T2 d2.
+Proof. intros Γ1 U du Γ2 Σ T1 d1 T2 d2 HST. remember (Γ1 ++ (U,du) :: Γ2) as Γ.
+  generalize dependent Γ1; induction HST; intros; intuition.
+  1,2: subst; constructor; auto; eapply narrowing_Qstp_gen; eauto.
+  - subst. constructor; auto. 1,2: eapply closed_ty_monotone; eauto; repeat rewrite app_length; simpl; auto. eapply narrowing_Qstp_gen; eauto.
+    unfold open_ty' in *. unfold openq' in *.
+    rewrite app_length in *. simpl in *.
+    repeat rewrite app_comm_cons.
+    eapply IHHST2; eauto.
+  - subst. specialize (IHHST1 Γ1).  specialize (IHHST2 Γ1). intuition.
+    specialize (H0 V dv).  specialize (H1 V dv). intuition.  eapply s_trans; eauto.
+Qed.
+
+Lemma narrowing_stp : forall{U du Γ Σ T1 d1 T2 d2}, stp ((U,du) :: Γ) Σ T1 d1 T2 d2 -> forall {V dv}, stp Γ Σ V dv U du -> stp ((V,dv) :: Γ) Σ T1 d1 T2 d2.
+  intros. specialize (@narrowing_stp_gen [] U du Γ Σ T1 d1 T2 d2) as narrow. simpl in *. eapply narrow; eauto.
+Qed.
+
+Lemma stp_scale_plus : forall {Γ Σ T1 d1 T2 d2}, stp Γ Σ T1 d1 T2 d2 -> forall {x}, x < length Γ -> stp Γ Σ T1 (d1 ⊕ x) T2 (d2 ⊕ x).
+  intros Γ Σ T1 d1 T2 d2 HSTP. induction HSTP; intros; econstructor; unfold_Q; nlift; unfold_N; intuition.
+Qed.
+
+Lemma saturated_empty : forall {Γ Σ}, saturated Γ Σ ∅.
+  intros. unfold saturated. intros. intuition.
+Qed.
+#[global] Hint Resolve saturated_empty : core.
+
+Lemma saturated_empty_tenv : forall {q Σ}, closed_Qual 0 0 (length Σ) (Q_lift q) -> saturated [] Σ q.
+  intros. unfold saturated. intros.
+  inversion H. subst. simpl in *. unfold_q. unfold N_lift in H0.
+  simpl in H0. apply H1 in H0. lia.
+Qed.
+#[global] Hint Resolve saturated_empty_tenv : core.
+
+Lemma saturated_cons : forall {Γ Σ q}, saturated Γ Σ q -> forall {T q'}, saturated ((T, q') :: Γ) Σ q.
+intros. unfold saturated in *. intros. apply H in H0. unfold saturated_var in *. destruct H0 as [U H0]. destruct H0 as [q0 H0]. intuition. exists U. exists q0. intuition. rewrite indexr_skip; eauto. apply indexr_var_some' in H1. lia.
+Qed.
+
+Lemma saturated_app : forall {Γ' Γ Σ q}, saturated Γ Σ q -> saturated (Γ' ++ Γ) Σ q.
+  induction Γ'; intros; simpl; intuition.
+  apply saturated_cons; auto.
+Qed.
+
+Lemma saturated_qplus : forall {Γ Σ x T q}, indexr x Γ = Some (T, q) -> closed_Qual 0 x (length Σ) (Q_lift q) -> saturated Γ Σ q -> saturated Γ Σ (q ⊕ x).
+  intros. unfold saturated. intros.
+qual_destruct q. unfold saturated,saturated_var in *. unfold_Q. nlift. unfold_N. intuition.
+  - specialize (H1 x0 H4). destruct H1 as [U [q' H1]]. exists U,q'. intuition.
+  - subst. exists T, (fvs, bvs, lcs). intuition.
+Qed.
+
+Lemma saturated_openq : forall {Γ Σ d1 d2}, saturated Γ Σ d1 -> saturated Γ Σ (openq ∅ d2) -> saturated Γ Σ (openq d1 d2).
+intros. qual_destruct d1. qual_destruct d2. unfold saturated, saturated_var, openq in *. intros. simpl in *. unfold_q.
+    ndestruct (bvs0 0); intuition. simpl in *. nlift. ndestruct (fvs x).
+  - specialize (H x H3). destruct H as [U [q' H]]. exists U,q'. unfold_Q. nlift. unfold_N. intuition.
+  - assert (H': N_or (N_lift fvs0) N_empty x). unfold_N. intuition. specialize (H0 x H'). destruct H0 as [U [q' H0]]. exists U,q'. unfold_Q. nlift. unfold_N. intuition.
+    + left. eapply H5 in H11. intuition.
+    + exfalso; eauto.
+    + left. eapply H9 in H11. intuition.
+Qed.
+
+Lemma saturated_qor : forall {Γ Σ q1 q2}, saturated Γ Σ q1 -> saturated Γ Σ q2 -> saturated Γ Σ (q1 ⊔ q2).
+intros. qual_destruct q1. qual_destruct q2. unfold saturated in *. intros. unfold saturated_var in *. simpl in *.
+unfold_q. nlift.
+ndestruct (fvs x).
+  - specialize (H x H2). destruct H as [U [q' H]]. exists U,q'. unfold_Q. nlift. unfold_N. intuition.
+  - assert (Hfvs0: N_lift fvs0 x). { unfold_N. intuition. }
+    specialize (H0 x Hfvs0). destruct H0 as [U [q' H0]]. exists U,q'. unfold_Q. nlift. unfold_N. intuition.
+Qed.
+
+Lemma saturated_just_loc : forall {Γ Σ l}, saturated Γ Σ (just_loc l).
+  intros. unfold saturated. intros. simpl in *.
+  unfold_q. unfold N_lift in *. unfold_n. discriminate.
+Qed.
+#[global] Hint Resolve saturated_just_loc : core.
+
+Lemma saturated_qand : forall {Γ Σ q1 q2}, saturated Γ Σ q1 -> saturated Γ Σ q2 -> saturated Γ Σ (q1 ⊓ q2).
+intros. qual_destruct q1. qual_destruct q2. unfold saturated in *. intros. unfold saturated_var in *. simpl in *.
+  assert (Hx : $ (x) ∈ᵥ (fvs, bvs, lcs) /\ $ (x) ∈ᵥ (fvs0, bvs0, lcs0)). {
+    simpl. unfold_Q. nlift. unfold_N. intuition.
+  }
+  intuition. simpl in *. apply H in H2. apply H0 in H3. destruct H2 as [U' [q' H2]]. destruct H3 as [U'' [q'' H3]]. intuition. rewrite H4 in H2. inversion H2. subst. exists U'',q''. intuition. unfold_Q. nlift. unfold_N. intuition.
+Qed.
+
+Lemma saturated_closed_Qual : forall {b Γ Σ q}, closed_Qual b 0 (length Σ) (Q_lift q) -> saturated Γ Σ q .
+intros. unfold saturated. intros. qual_destruct q. unfold_q. exfalso. Qcrush. intuition eauto.
+Qed.
+
+Lemma weaken_store_saturated : forall {Γ Σ q}, saturated Γ Σ q -> forall {Σ'}, Σ' ⊇ Σ -> saturated Γ Σ' q.
+  intros. unfold saturated in *. intros. specialize (H x H1).
+  unfold saturated_var in *. destruct H as [U [q' H]]. exists U. exists q'. intuition. unfold_Q. intuition. eapply closed_Nats_mono; eauto. apply extends_length; auto.
+Qed.
+
+Lemma wf_tenv_empty : forall {Σ}, wf_tenv [] Σ.
+  unfold wf_tenv. intros. simpl in H. discriminate.
+Qed.
+#[global] Hint Resolve wf_tenv_empty : core.
+
+Lemma wf_tenv_cons : forall {Γ Σ}, wf_tenv Γ Σ -> forall {T q}, saturated Γ Σ q -> wf_tenv ((T, q) :: Γ) Σ.
+  intros. unfold wf_tenv. intros. bdestruct (x =? (length Γ)).
+  - subst. rewrite indexr_head in H1. inversion H1. subst. apply saturated_cons. auto.
+  - rewrite indexr_skip in H1; auto. apply H in H1. apply saturated_cons. auto.
+Qed.
+
+Fixpoint has_type_closed  {Γ φ Σ t T d} (ht : has_type Γ φ Σ t T d) :
+  closed_Qual 0 (length Γ) (length Σ) (Q_lift φ) /\
+  closed_tm 0 (length Γ) (length Σ) t /\
+  closed_ty 0 (length Γ) (length Σ) T /\
+  closed_Qual 0 (length Γ) (length Σ) (Q_lift d).
+Proof.
+  destruct ht; intuition; try apply has_type_closed in ht; try apply has_type_closed in ht1;
+  try apply has_type_closed in ht2; simpl in *; intuition eauto.
+  - apply indexr_var_some' in H. auto.
+  - apply indexr_var_some' in H.
+    eapply closed_ty_monotone; eauto. lia.
+  - apply indexr_var_some' in H.
+    eapply qplus_closed_qual; eauto. lia.
+  - unfold_Q. unfold_N. intuition eauto.
+  - unfold openq in *. rewrite Q_lift_open_qual. qual_destruct d1. qual_destruct d2. unfold_Q. unfold_N. unfold_q.
+    (* NOTE: requires some complex strategy <2023-05-22, David Deng> *)
+    ndestruct (bvs0 0); intuition.
+  - apply indexr_var_some' in H0. auto.
+  - unfold_Q. unfold_q. rewrite N_lift_one,N_lift_empty in *. intuition eauto.
+  - eapply closed_ty_monotone; eauto; lia.
+  - apply stp_closed in H. intuition.
+  - apply stp_closed in H. intuition.
+Qed.
+
+Lemma openq_subqual : forall {d1 d2 φ}, Subq (Q_lift d1) (Q_lift φ) -> Subq (Q_lift (openq ∅ d2)) (Q_lift φ) -> Subq (Q_lift (openq d1 d2)) (Q_lift φ).
+intros. qual_destruct d1. qual_destruct d2. qual_destruct φ. unfold openq in *. rewrite Q_lift_open_qual in *. unfold_Q. unfold_N. unfold_q.
+ndestruct (bvs0 0); intuition.
+Qed.
+
+Fixpoint has_type_filter {Γ φ Σ t T d} (ht : has_type Γ φ Σ t T d) : d ⊑↑ φ.
+destruct ht; try apply subq_empty. all: try apply openq_subqual; eauto.
+Qed.
+
+Fixpoint has_type_saturated {Γ φ Σ t T d} (wfG : wf_tenv Γ Σ) (ht : has_type Γ φ Σ t T d) : saturated Γ Σ d.
+  destruct ht; intuition. eapply saturated_qplus; eauto.
+  apply saturated_openq; auto. apply has_type_saturated in ht2; auto.
+Qed.
+
+Lemma indexr_splice_tenv : forall {Γ1 i Γ2 U du},
+    indexr i (Γ1 ++ Γ2) = Some (U, du) ->
+    forall {k}, k <= i -> (length Γ2) <= i -> indexr i (splice_tenv k Γ1 ++ Γ2) = Some (splice_ty k U, splice_qual k du).
+  induction Γ1; intros; simpl in *; intuition. apply indexr_var_some' in H. lia.
+  rewrite app_length in *. rewrite splice_tenv_length.
+  destruct (Nat.eqb i (length Γ1 + length Γ2)) eqn:Heq. inversion H. subst.
+  simpl. auto. apply IHΓ1; eauto.
+Qed.
+
+Lemma weaken_saturated : forall {Γ1 Γ2 Σ d1},
+    saturated (Γ1 ++ Γ2) Σ d1 ->
+    let k := (length Γ2) in forall X, saturated ((splice_tenv k Γ1) ++ X :: Γ2) Σ (splice_qual k d1).
+  intros. unfold saturated. intros. bdestruct (x <? k).
+  - specialize (H x). apply splice_qual_mem_lt in H0; auto. intuition. unfold saturated_var in *. destruct H2 as [U H2]. destruct H2 as [q0 H2]. exists U. exists q0. intuition.
+    rewrite indexr_skips in H; try lia.
+    rewrite indexr_skips. rewrite indexr_skip; auto. lia. simpl. lia.
+    replace q0 with (splice_qual k q0). repeat rewrite Q_lift_splice_qual. unfold_Q. intuition.
+    eapply splice_qual_id. eapply closed_Qual_monotone; eauto. lia.
+  - bdestruct (x =? k).
+    + subst. simpl in *. qual_destruct d1. unfold_q. rewrite N_lift_splice in H0. unfold_N. intuition.
+    + destruct x. lia. specialize (H x). assert (Hx : x >= k). lia.
+      assert ($ (x) ∈ᵥ d1). qual_destruct d1. unfold_q. rewrite N_lift_splice in H0. unfold_N. intuition.
+simpl in *. intuition. unfold saturated_var in *. intuition.
+      destruct H4 as [U H4]. destruct H4 as [q0 H4].
+      exists (splice_ty k U). exists (splice_qual k q0). intuition. eapply indexr_splice_tenv; eauto. rewrite <- indexr_insert_ge; eauto. simpl. lia. all: repeat rewrite Q_lift_splice_qual; unfold_Q; intuition.
+Qed.
+
+Lemma weaken_gen : forall {t Γ1 Γ2 φ Σ T d},
+    has_type (Γ1 ++ Γ2) φ Σ t T d ->
+    let k := (length Γ2) in
+    forall X, has_type ((splice_tenv k Γ1) ++ X :: Γ2) (splice_qual k φ) Σ (splice k t) (splice_ty k T) (splice_qual k d).
+  intros t Γ1 Γ2 φ Σ T d HT. remember (Γ1 ++ Γ2) as Γ. generalize dependent Γ1. generalize dependent Γ2.
+  induction HT; intros; subst.
+  - (* tunit *) simpl. rewrite n_splice_id; eauto. constructor.
+    qual_destruct φ. rewrite Q_lift_splice_qual. rewrite app_length in *. rewrite splice_tenv_length. unfold_Q. intuition. rewrite <- plus_n_Sm. eauto using N_splice_closed. unfold_n. intuition.
+  - (* t_var *)
+    (* simpl. *)
+    destruct (le_lt_dec k x) eqn:Heq.
+    + (* |Γ2| <= x < |Γ1|+|Γ2|*)
+      erewrite <- splice_qual_qplus_dist; eauto. simpl. rewrite Heq. constructor.
+      rewrite <- indexr_insert_ge. apply indexr_splice_tenv; eauto. lia.
+      rewrite splice_qual_qplus_dist; try lia. repeat rewrite Q_lift_splice_qual. rewrite Subq_splice_dist. auto.
+rewrite Q_lift_splice_qual. qual_destruct φ. unfold_Q. rewrite app_length in *. rewrite splice_tenv_length. simpl. rewrite <- plus_n_Sm. intuition. apply splice_ty_closed''; intuition.
+      rewrite Q_lift_splice_qual. unfold_Q. intuition.
+    + (* |Γ2| > x *)
+      erewrite splice_qual_qplus_id; eauto. simpl. rewrite Heq. constructor.
+      rewrite <- indexr_insert_lt; auto. rewrite indexr_skips; auto.
+      rewrite indexr_skips in H; auto.
+      erewrite splice_ty_id. auto.
+      eapply closed_ty_monotone; eauto. lia.
+      1,2: rewrite Q_lift_splice_qual.
+      erewrite <- @splice_Qual_qplus_id with (k:=k); eauto. rewrite <- @Subq_splice_dist with (i:=k) in H0; auto.
+      rewrite app_length in *. rewrite splice_tenv_length. qual_destruct φ. unfold_Q. unfold_N. intuition. bdestruct (x0<?k); intuition. assert (x0 > k) by lia. intuition. apply H0 in H15. lia.
+      erewrite splice_ty_id; eauto. auto.
+  - (* t_abs *) rewrite app_length in *. simpl. constructor.
+    apply splice_closed'.
+    1-3: rewrite app_length; rewrite splice_tenv_length; simpl. auto.
+    1,2: repeat rewrite <- plus_n_Sm.
+    1-3: repeat rewrite Q_lift_splice_qual.
+    simpl in H0. intuition; unfold_Q; intuition; apply splice_ty_closed''; eauto; lia.
+    1,2: unfold_Q; intuition.
+    1,2: apply weaken_saturated; auto.
+    rewrite app_comm_cons.
+    replace ((splice_ty k T1, splice_qual k d1) :: splice_tenv k Γ1) with (splice_tenv k ((T1, d1) :: Γ1)); auto.
+    replace (splice_qual k df ⊔ just_fv (length (splice_tenv k Γ1 ++ X :: Γ2)))
+            with (splice_qual k (df ⊔ just_fv (length Γ1 + length Γ2))).
+    subst k. rewrite <- splice_tm_open'. rewrite <- splice_ty_open'. rewrite <- splice_qual_open'.
+    rewrite @open_tm'_len with (Γ':=(Γ1 ++ Γ2)). rewrite @open_ty'_len with (Γ':=(Γ1 ++ Γ2)).
+    rewrite @openq'_len with (Γ':=(Γ1 ++ Γ2)).
+    apply IHHT; intuition. 1-4 : repeat rewrite app_length; rewrite splice_tenv_length; auto. replace (length Γ1 + length (X :: Γ2)) with (length Γ1 + S (length Γ2)) by auto. rewrite <- plus_n_Sm. rewrite splice_qual_qplus_dist. unfold qor. unfold qor. auto. lia.
+  - (* tapp *) simpl. rewrite splice_qual_open''. apply t_app with (T1:=(splice_ty k T1)) (df:=(splice_qual k df)).
+    replace (TFun (splice_qual k df ⊓ splice_qual k d1)  (splice_qual k d2) (splice_ty k T1) (splice_ty k T2)) with
+    (splice_ty k (TFun (df ⊓ d1) d2 T1 T2)); auto.
+    apply IHHT1; auto. simpl. f_equal. rewrite <- splice_qual_qand_dist.
+(* NOTE: Q: define a lemma? unfold? <2023-05-23, David Deng> *)
+    unfold_q. repeat f_equal.
+    apply IHHT2; auto.
+    eapply splice_ty_closed'. rewrite app_length in *. rewrite splice_tenv_length. auto.
+    1,2 : subst k; rewrite <- @splice_qual_empty with (k := length Γ2); rewrite <- splice_qual_open''.
+    repeat rewrite Q_lift_splice_qual. rewrite Subq_splice_dist; auto.
+    apply weaken_saturated; auto.
+  - (* t_loc *) simpl. rewrite n_splice_id. constructor. rewrite Q_lift_splice_qual.
+    eapply splice_qual_closed'. rewrite app_length in *. rewrite splice_tenv_length. unfold_Q. intuition.
+    1,2: erewrite splice_ty_id; eauto; eapply closed_ty_monotone; eauto; lia.
+    rewrite Q_lift_splice_qual. unfold_Q. intuition. rewrite N_lift_empty. unfold_N. intuition.
+    unfold_n. intuition.
+  - (* t_ref *) simpl. rewrite n_splice_id. eapply t_ref. simpl in IHHT. specialize (IHHT Γ2 Γ1). intuition. unfold_n. intuition.
+  - (* t_deref *) simpl. rewrite n_splice_id. econstructor. simpl in IHHT. subst k. apply IHHT; auto. unfold_n. intuition.
+  - (* t_assign *) replace (splice_qual k ∅) with (∅) by auto. replace (splice_ty k TUnit) with (TUnit) by auto. simpl. eapply t_assign.
+    1-2: replace (∅) with (splice_qual k ∅) by auto.
+    replace (TRef TUnit) with (splice_ty k (TRef TUnit)) by auto. apply IHHT1; auto.
+    replace (TUnit) with ((splice_ty k TUnit)) by auto. apply IHHT2; auto.
+  - (* t_sub *) eapply t_sub. eapply IHHT; auto.
+    apply @weaken_stp_gen; eauto; lia. apply subq_splice_dist. auto.
+    apply weaken_saturated; auto.
+Qed.
+
+Lemma weaken_flt : forall {Γ φ Σ t T d},
+    has_type Γ φ Σ t T d ->
+    forall {φ'}, Subq (Q_lift φ) (Q_lift φ') ->
+                 closed_Qual 0 (length Γ) (length Σ) (Q_lift φ') ->
+    has_type Γ φ' Σ t T d.
+  intros Γ φ Σ t T d HT. induction HT; intros; econstructor; eauto; unfold_Q; intuition; nlift; unfold_N; intuition.
+Qed.
+
+Lemma weaken : forall {φ Σ t T d},
+    has_type [] φ Σ t T d -> forall {Γ}, has_type Γ φ Σ t T d.
+  intros φ Σ t T d HT. induction Γ; auto.
+  specialize (@weaken_gen t [] Γ φ Σ T d) as Hsp. simpl in *.
+  specialize (Hsp IHΓ a).
+  apply has_type_closed in HT. intuition. simpl in *.
+  replace (splice (length Γ) t) with t in Hsp.
+  replace (splice_ty (length Γ) T) with T in Hsp.
+  replace (splice_qual (length Γ) d) with d in Hsp.
+  replace (splice_qual (length Γ) φ) with φ in Hsp. auto.
+  all : symmetry.
+  eapply splice_qual_id; eauto. eapply closed_Qual_monotone; eauto; lia.
+  eapply splice_qual_id; eauto. eapply closed_Qual_monotone; eauto; lia.
+  eapply splice_ty_id; eauto.   eapply closed_ty_monotone; eauto; lia.
+  eapply splice_tm_id; eauto.      eapply closed_tm_monotone; eauto; lia.
+Qed.
+
+Lemma weaken' : forall {φ Σ t T d},
+    has_type [] φ Σ t T d -> forall {φ'}, Subq (Q_lift φ) (Q_lift φ') -> forall {Γ}, closed_Qual 0 (length Γ) (length Σ) (Q_lift φ') -> has_type Γ φ' Σ t T d.
+  intros. eapply weaken_flt; eauto. apply weaken. eauto.
+Qed.
+
+Lemma weaken_store : forall {Γ φ Σ t T d}, has_type Γ φ Σ t T d -> forall {Σ'}, Σ' ⊇ Σ -> has_type Γ φ Σ' t T d.
+  intros Γ φ Σ t T d HT.
+  induction HT; intros; intuition; econstructor; eauto;
+    try solve [unfold_Q; intuition; eapply closed_Nats_mono; eauto; apply extends_length; eauto];
+    try solve [eapply closed_qual_monotone; eauto; apply extends_length; auto];
+    try solve [eapply closed_tm_monotone; eauto; apply extends_length; auto];
+    try solve [eapply closed_ty_monotone; eauto; apply extends_length; auto];
+    try solve [eapply weaken_store_saturated; eauto].
+  - unfold extends in H3. destruct H3. rewrite H3.
+    rewrite indexr_skips. auto. eapply indexr_var_some'. eauto.
+  - eapply weaken_stp_store_ext; eauto.
+Qed.
+
+Lemma values_stuck : forall {v}, value v -> forall {t σ σ'}, step v σ t σ' -> False.
+  intros. inversion H0; subst; inversion H.
+Qed.
+
+Lemma CtxOK_ext : forall {Γ φ Σ σ}, CtxOK Γ φ Σ σ -> forall {v T}, has_type Γ φ Σ v T ∅ -> value v -> CtxOK Γ φ (T :: Σ) (v :: σ).
+  intros. unfold CtxOK in *. split. simpl. lia.
+  intros. destruct H as [Hlen Hprev]. destruct (Nat.eqb l (length σ)) eqn:Heql.
+  - simpl in *. rewrite Heql in *. inversion H3. subst.
+    rewrite <- Hlen in Heql. rewrite Heql in H2. inversion H2. subst. intuition.
+    eapply weaken_store; eauto. apply extends_cons.
+  - simpl in *. rewrite Heql in *. rewrite <- Hlen in Heql. rewrite Heql in H2.
+    specialize (Hprev _ _ _ H2 H3) as Hprev. intuition.
+    eapply weaken_store; eauto. apply extends_cons.
+Qed.
+
+Lemma CtxOK_update : forall {Γ φ Σ σ}, CtxOK Γ φ Σ σ -> forall {l T}, l < length σ -> indexr l Σ = Some T -> forall {v}, has_type Γ φ Σ v T ∅ -> value v -> CtxOK Γ φ Σ (update σ l v).
+  intros. unfold CtxOK in *. destruct H as [Hlen Hprev].
+  split. rewrite <- update_length. auto.
+  intros. destruct (Nat.eqb l l0) eqn:Heq.
+  - apply Nat.eqb_eq in Heq. subst.
+    apply (@update_indexr_hit _ σ l0 v) in H0. rewrite H1 in H. inversion H. subst.
+    rewrite H4 in H0. inversion H0. subst. intuition.
+  - apply Nat.eqb_neq in Heq. apply (@update_indexr_miss _ σ l v l0) in Heq.
+    rewrite Heq in H4. eapply Hprev; eauto.
+Qed.
+
+Lemma CtxOK_empty : forall {Γ φ}, CtxOK Γ φ [] [].
+  intros. constructor; intuition; simpl in H; try discriminate.
+Qed.
+#[global] Hint Resolve CtxOK_empty : core.
+
+Lemma CtxOK_weaken_flt : forall {Γ φ Σ σ}, CtxOK Γ φ Σ σ -> forall {φ'}, closed_Qual 0 (length Γ) (length Σ) (Q_lift φ') -> φ ⊑↑ φ' -> CtxOK Γ φ' Σ σ.
+  intros. inversion H. subst. constructor; intuition.
+  all : specialize (H3 _ _ _ H4 H5); intuition.
+  eapply weaken_flt; eauto.
+Qed.
+
+Lemma subst1_tenv_length : forall {v q Γ}, length ({ v |-> q }ᴳ Γ) = length Γ.
+  intros. unfold subst_tenv. rewrite map_length. auto.
+Qed.
+
+Lemma subst_tenv_length : forall {v q q' Γ}, length ({ v |-> q ; q' }ᴳ Γ) = length Γ.
+  intros. repeat rewrite subst1_tenv_length. auto.
+Qed.
+
+Lemma subst1_ty_id : forall {T b l}, closed_ty b 0 l T -> forall {d1}, { 0 |-> d1 }ᵀ T = T.
+induction T; intros; simpl in *; auto; intuition;
+                       try solve [erewrite IHT; eauto];
+                       try solve [erewrite IHT1; eauto; erewrite IHT2; eauto].
+  erewrite IHT1; eauto. erewrite IHT2; eauto.
+  erewrite subst1_qual_id; eauto. erewrite subst1_qual_id; eauto.
+Qed.
+
+Lemma subst_ty_id : forall {b l T}, closed_ty b 0 l T -> forall {d1 d2}, { 0 |-> d1 ; d2 }ᵀ T = T.
+  intros. repeat erewrite subst1_ty_id; eauto.
+Qed.
+
+Lemma subst1_tm_id : forall {t b l}, closed_tm b 0 l t -> forall {t1}, { 0 |-> t1 }ᵗ t = t.
+induction t; intros; simpl in *; intuition;
+                       try solve [erewrite IHt; eauto];
+                       try solve [erewrite IHt1; eauto; erewrite IHt2; eauto].
+destruct v; intuition.
+Qed.
+
+Lemma open_subst1_qual : forall {q b l},
+    closed_Qual b 0 l (Q_lift q) ->
+    forall {k d1},
+    [[k ~> d1 ]]ᵈ q = { 0 |-> d1 }ᵈ ([[k ~> (just_fv 0)]]ᵈ q).
+intros. qual_destruct d1. qual_destruct q. unfold_Q. unfold_q.
+destruct (bvs0 k) eqn:Eq; simpl; f_equal.
+- assert (Ht: n_or fvs0 (n_one 0) 0 = true). { apply (proj1 (reflect_iff _ _ (n_reflect_true _ _))). nlift. unfold_N. intuition. } rewrite Ht. apply Q_lift_eq. unfold_Q. nlift. unfold_N. repeat f_equal; apply functional_extensionality; intros; apply propositional_extensionality; intuition. exfalso; eauto 3 with arith.
+- destruct (fvs0 0) eqn:Eq2; apply Q_lift_eq; unfold_Q; nlift; unfold_N; repeat f_equal; apply functional_extensionality; intuition; apply propositional_extensionality; intuition. all: exfalso; eauto 3 with arith.
+Qed.
+
+Lemma open_subst1_ty : forall {T b l},
+    closed_ty b 0 l T ->
+    forall {k d1},
+      [[k ~> d1 ]]ᵀ T = { 0 |-> d1 }ᵀ ([[k ~> (just_fv 0)]]ᵀ T).
+  induction T; intros; simpl in *; intuition.
+  erewrite IHT1; eauto. erewrite IHT2; eauto.
+  erewrite <- open_subst1_qual; eauto. erewrite <- open_subst1_qual; eauto.
+  erewrite IHT; eauto.
+Qed.
+
+Lemma open_subst1_tm : forall {t b l},
+    closed_tm b 0 l t ->
+    forall {k b' l' t1},
+      closed_tm b' 0 l' t1 ->
+      [[k ~> t1 ]]ᵗ t = { 0 |-> t1 }ᵗ ([[k ~> $ 0]]ᵗ t).
+induction t; intros b loc Hc; intros; simpl in *; intuition;
+    try solve [erewrite IHt; eauto];
+    try solve [erewrite IHt1; eauto; erewrite IHt2; eauto].
+  destruct v; intuition. bdestruct (k =? i); simpl; intuition.
+Qed.
+
+Fixpoint open_subst1_tm_comm {t : tm} :
+  forall {k  g tf ff lf}, closed_tm 0 ff lf tf ->
+    [[k ~> $ (g) ]]ᵗ ({0 |-> tf }ᵗ t) = {0 |-> tf }ᵗ ([[ k ~> $ (S g) ]]ᵗ  t).
+    destruct t; intros; simpl; intuition;
+      try solve [repeat erewrite open_subst1_tm_comm; eauto].
+    destruct v; simpl.
+    bdestruct (i =? 0); simpl. eapply closed_tm_open_id; eauto. lia. auto.
+    bdestruct (k =? i); simpl; auto.
+Qed.
+
+Lemma open_subst1_qual_comm : forall {q : qual} {k g df ff lf},
+    closed_Qual 0 ff lf (Q_lift df) ->
+    [[k ~> just_fv g ]]ᵈ ({0 |-> df }ᵈ q) = {0 |-> df }ᵈ ([[ k ~> just_fv (S g) ]]ᵈ q).
+  intros. qual_destruct df. qual_destruct q. unfold_q.
+  ndestruct (fvs0 0); ndestruct (bvs0 k); simpl.
+  - ndestruct (n_or bvs0 bvs k); ndestruct (n_or fvs0 (n_one (S g)) 0); apply Q_lift_eq; unfold_Q; nlift; unfold_N; repeat f_equal; apply functional_extensionality; intros; apply propositional_extensionality; intuition. all: exfalso; eauto.
+  - ndestruct (n_or bvs0 bvs k); ndestruct (fvs0 0); apply Q_lift_eq; unfold_Q; nlift; unfold_N; repeat f_equal; apply functional_extensionality; intros; apply propositional_extensionality; intuition. all: exfalso; eauto.
+  - ndestruct (bvs0 k); ndestruct (n_or fvs0 (n_one (S g)) 0); apply Q_lift_eq; unfold_Q; nlift; unfold_N; repeat f_equal; apply functional_extensionality; intros; apply propositional_extensionality; intuition. all: exfalso; eauto.
+  - ndestruct (bvs0 k); ndestruct (fvs0 0); apply Q_lift_eq; unfold_Q; nlift; unfold_N; repeat f_equal; apply functional_extensionality; intros; apply propositional_extensionality; intuition. all: exfalso; eauto.
+Qed.
+
+Lemma open_subst1_qual_comm2 : forall {q : qual} {k g df ff lf},
+    closed_Qual 0 ff lf (Q_lift df) ->
+    [[k ~> just_fv g ]]ᵈ ({0 |-> df }ᵈ q) = {0 |-> df }ᵈ ([[ k ~> just_fv (S g) ]]ᵈ q).
+ intros. apply Q_lift_eq. repeat rewrite Q_lift_subst_qual,Q_lift_open_qual. unfold_Q. nlift. unfold_N.
+repeat f_equal; apply functional_extensionality; intros; apply propositional_extensionality.
+- split. intros. split. intros.
+  (* intuition *)
+  (* runs forever *)
+  (* TODO: better way? <2023-06-01, David Deng> *)
+Admitted.
+
+Fixpoint open_subst1_ty_comm {T : ty} :
+  forall {k g df ff lf}, closed_qual 0 ff lf df ->
+    [[k ~> just_fv g ]]ᵀ ({0 |-> df }ᵀ T) = {0 |-> df }ᵀ ([[ k ~> just_fv (S g) ]]ᵀ  T).
+    destruct T; intros; simpl; intuition;
+      try solve [repeat erewrite open_subst1_ty_comm; eauto].
+    erewrite open_subst1_qual_comm; eauto.
+    erewrite open_subst1_qual_comm; eauto.
+    erewrite open_subst1_ty_comm; eauto.
+    erewrite open_subst1_ty_comm; eauto.
+Qed.
+
+Lemma closed_Qual_subst1 : forall {q b f l},
+    closed_Qual b (S f) l (Q_lift q) ->
+    forall {d1 l1}, closed_Qual 0 0 l1 (Q_lift d1) ->
+    forall{l2},
+      l <= l2 -> l1 <= l2 ->
+      closed_Qual b f l2 (Q_lift ({0 |-> d1}ᵈ q)).
+  intros. rewrite Q_lift_subst_qual. unfold_Q. unfold_N. intuition; nlem; intuition;
+  try solve [ exfalso; eauto ];
+  try solve [ eauto using lt_S_n,Nat.lt_le_trans ].
+Qed.
+
+Lemma closed_ty_subst1 : forall {T b f l},
+    closed_ty b (S f) l T ->
+    forall {d1 l1}, closed_Qual 0 0 l1 (Q_lift d1) ->
+    forall{l2},
+      l <= l2 -> l1 <= l2 ->
+      closed_ty b f l2 ({0 |-> d1}ᵀ T).
+  intros T b f l Hc. remember (S f) as f'. generalize dependent f. generalize dependent b.
+  induction T; intros; subst; simpl in *; intuition.
+  1,2: eapply closed_Qual_subst1; eauto.
+  eapply IHT1; eauto.
+  eapply IHT2; eauto; lia.
+  erewrite subst1_ty_id; eauto.
+Qed.
+
+Lemma closed_tm_subst1 : forall {t b f l},
+    closed_tm b (S f) l t ->
+    forall {t1 l1}, closed_tm 0 0 l1 t1 ->
+    forall{l2},
+      l <= l2 -> l1 <= l2 ->
+      closed_tm b f l2 ({0 |-> t1}ᵗ t).
+  intros t b f l Hc. remember (S f) as f'.
+  generalize dependent f.
+  generalize dependent b.
+  induction t; intros; subst; simpl in *; intuition; try constructor;
+    try solve [eapply IHt; eauto; lia ];
+    try solve [eapply IHt1; eauto];
+    try solve [eapply IHt2; eauto].
+  destruct v; auto. bdestruct (i =? 0).
+  eapply closed_tm_monotone; eauto; lia. simpl; lia.
+Qed.
+
+Lemma subst1_qor_dist : forall {q1 q2 df},
+    ({ 0 |-> df }ᵈ (q1 ⊔ q2)) = (({ 0 |-> df }ᵈ q1) ⊔ ({ 0 |-> df }ᵈ q2)).
+intros. qual_destruct q1. qual_destruct q2. unfold subst_qual. unfold_q.
+ndestruct (n_or fvs fvs0 0); ndestruct (fvs 0); ndestruct (fvs0 0); apply Q_lift_eq;
+unfold_Q; nlift; unfold_N; repeat f_equal; apply functional_extensionality; intros; apply propositional_extensionality; intuition.
+Qed.
+
+Lemma subst1_qual_plus_dist : forall {x d df},
+    1 <= x -> ({ 0 |-> df }ᵈ (d ⊕ x)) = (({ 0 |-> df }ᵈ d) ⊕ (pred x)).
+Proof.
+  intros. qual_destruct d; qual_destruct df. simpl. apply Q_lift_eq. repeat rewrite Q_lift_or,Q_lift_subst_qual. unfold_Q. nlift. unfold_N. repeat f_equal; apply functional_extensionality; intros; apply propositional_extensionality; intuition.
+  ndestruct (fvs 0); intuition.
+Qed.
+
+Lemma indexr_subst1 : forall {x Γ T U d dx},
+    x >= 1 ->
+    indexr x (Γ ++ [U]) = Some (T, d) ->
+    indexr (pred x) ({ 0 |-> dx }ᴳ Γ) = Some ({ 0 |-> dx }ᵀ T, { 0 |-> dx }ᵈ d).
+  intros. destruct x; try lia.
+  rewrite <- indexr_insert_ge in H0; simpl; try lia.
+  rewrite app_nil_r in H0. induction Γ; intros; simpl in *. discriminate.
+  rewrite subst1_tenv_length. (bdestruct (x =? length Γ)); auto.
+  inversion H0. auto.
+Qed.
+
+Lemma closed_qual_subst1' : forall {Γ0 X l df φ b},
+    closed_Qual 0 0 l (Q_lift df) ->
+    closed_Qual b (length (Γ0 ++ [X])) l (Q_lift φ) ->
+    closed_Qual b (length ({0 |-> df }ᴳ Γ0)) l (Q_lift ({0 |-> df }ᵈ φ)).
+  intros. eapply closed_Qual_subst1; eauto. rewrite subst1_tenv_length.
+  rewrite app_length in *. simpl in *. replace (length Γ0 + 1) with (S (length Γ0)) in H0 by lia. auto.
+Qed.
+
+Lemma closed_tm_subst1' : forall {Γ0 X l df tx t b},
+    closed_tm 0 0 l tx ->
+    closed_tm b (length (Γ0 ++ [X])) l t ->
+    closed_tm b (length ({0 |-> df }ᴳ Γ0)) l ({0 |-> tx }ᵗ t).
+  intros. eapply closed_tm_subst1; eauto. rewrite subst1_tenv_length.
+  rewrite app_length in *. simpl in *. replace (length Γ0 + 1) with (S (length Γ0)) in H0.
+  auto. lia.
+Qed.
+
+Lemma closed_ty_subst1' : forall {Γ0 X l df T b},
+    closed_qual 0 0 l df ->
+    closed_ty b (length (Γ0 ++ [X])) l T ->
+    closed_ty b (length ({0 |-> df }ᴳ Γ0)) l ({0 |-> df }ᵀ T).
+  intros. repeat eapply closed_ty_subst1; eauto. rewrite subst1_tenv_length.
+  rewrite app_length in *. simpl in *. replace (length Γ0 + 1) with (S (length Γ0)) in H0.
+  auto. lia.
+Qed.
+
+Lemma subst_qstp :  forall {gl df' sl d1 d2},
+    Qstp (S gl) sl (Q_lift d1) (Q_lift d2) ->
+    closed_Qual 0 0 sl (Q_lift df') ->
+    (* Substq df df' -> *)
+    Qstp gl sl (Q_lift ({0 |-> df' }ᵈ d1)) (Q_lift ({0 |-> df' }ᵈ d2)).
+  intros. qual_destruct d1. qual_destruct d2. qual_destruct df'. repeat rewrite Q_lift_subst_qual. unfold_Q. unfold_N. intuition.
+  all: nlem; intuition; eauto using lt_S_n. exfalso. eauto.
+Qed.
+
+Lemma subst_stp : forall{T1 T2},
+    forall {Γ Tf df df' Σ d1 d2},
+      stp (Γ ++ [(Tf,df)]) Σ T1 d1 T2 d2 ->
+      closed_qual 0 0 (length Σ) df' ->
+      (* Substq' (Q_lift df') (Q_lift df) -> *)
+      stp ({ 0 |-> df' }ᴳ Γ) Σ
+          ({ 0 |-> df' }ᵀ T1) ({ 0 |-> df' }ᵈ d1)
+          ({ 0 |-> df' }ᵀ T2) ({ 0 |-> df' }ᵈ d2).
+  intros T1 T2 Γ Tf df df' Σ d1 d2 HS.
+  remember (Γ ++ [(Tf, df)]) as Γ'.
+  generalize dependent Γ. generalize dependent df.  generalize dependent Tf. induction HS; intros; subst.
+- simpl. constructor. rewrite app_length in H. simpl in H. rewrite Nat.add_1_r in H. rewrite subst1_tenv_length. eapply subst_qstp; simpl in *; eauto.
+- specialize (stp_closed HS1). specialize (stp_closed HS2). intuition. simpl. constructor. rewrite app_length in H. simpl in H. rewrite Nat.add_1_r in H. rewrite subst1_tenv_length. eapply subst_qstp; simpl in *; eauto. all : repeat erewrite subst1_ty_id; eauto.
+- intuition. rewrite app_length in *. simpl in *. rewrite Nat.add_1_r in *. constructor; simpl; intuition; try rewrite subst1_tenv_length;
+  try solve [eapply closed_Qual_subst1; eauto];
+  try solve [eapply closed_ty_subst1; eauto].
+  eapply subst_qstp; eauto. eapply IHHS1; eauto.
+  unfold open_ty' in *. unfold open_ty in *.
+  unfold openq' in *. unfold openq in *.
+  rewrite app_length in *. rewrite subst1_tenv_length. simpl in *.
+  replace (length Γ0 + 1) with (S (length Γ0)) in *; try lia.
+  specialize (IHHS2 Tf df ((T3, d3) :: Γ0)). simpl in IHHS2. intuition. rename H10 into IHHS2.
+  erewrite <- open_subst1_ty_comm in IHHS2; eauto. erewrite <- open_subst1_ty_comm in IHHS2; eauto.
+  erewrite <- open_subst1_qual_comm in IHHS2; eauto. erewrite <- open_subst1_qual_comm in IHHS2; eauto.
+  -  econstructor; eauto.
+Qed.
+
+Lemma substitution_stp : forall{T1 T2},
+    forall {Tf df dx Σ d1 d2},
+      stp ([(Tf,df ⊓ dx)]) Σ T1 d1 T2 d2 -> closed_qual 0 0 (length Σ) dx ->
+      stp [] Σ ({ 0 |-> dx }ᵀ T1) ({ 0 |-> dx }ᵈ d1) ({ 0 |-> dx }ᵀ T2) ({ 0 |-> dx }ᵈ d2).
+  intros. replace [(Tf, df ⊓ dx)] with ([] ++ [(Tf, df ⊓ dx)]) in H; auto.
+  replace [] with ({0 |-> dx }ᴳ []); auto.
+  eapply subst_stp; eauto.
+Qed.
+
+Lemma subst1_just_fv0 : forall {q}, {0 |-> q }ᵈ (just_fv 0) = q.
+  intros. apply Q_lift_eq. unfold_Q. nlift. unfold_N. repeat f_equal; apply functional_extensionality; intros; apply propositional_extensionality; intuition.
+Qed.
+
+Lemma subst1_preserves_separation : forall {df d1 Tx dx dx' Γ Σ φ},
+    dx' ⊓ φ = dx ->
+    closed_Qual 0 0 (length Σ) (Q_lift dx') ->
+    df ⊑↑ φ -> d1 ⊑↑ φ ->
+    saturated (Γ ++ [(Tx, dx)]) Σ d1 ->
+    saturated (Γ ++ [(Tx, dx)]) Σ df ->
+    {0 |-> dx' }ᵈ df ⊓ {0 |-> dx' }ᵈ d1 = {0 |-> dx' }ᵈ (df ⊓ d1).
+  intros. qual_destruct df. qual_destruct d1. unfold_q.
+  unfold saturated,saturated_var,qmem in *.
+ndestruct (fvs 0); ndestruct (fvs0 0); ndestruct (n_and fvs fvs0 0); apply Q_lift_eq; unfold_Q; nlift; unfold_N; unfold N_lift in H; repeat f_equal; apply functional_extensionality; intros; apply propositional_extensionality; intuition.
+  - exfalso; eauto.
+  - specialize (H4 0). intuition. destruct H15 as [U' [q' H15]]. intuition. assert (Hl0: 0 = (length ([]: tenv))). auto. rewrite Hl0 in H4. rewrite indexr_insert in H4. inversion H4. subst. simpl in *. nlift. unfold_N. intuition.
+  - exfalso; eauto.
+  - specialize (H3 0). intuition. destruct H16 as [U' [q' H16]]. intuition. assert (Hl0: 0 = (length ([]: tenv))). auto. rewrite Hl0 in H3. rewrite indexr_insert in H3. inversion H3. subst. simpl in *. nlift. unfold_N. intuition.
+Qed.
+
+Lemma subst1_mem : forall {x dx df l}, closed_Qual 0 0 l (Q_lift dx) -> $ (x) ∈ᵥ {0 |-> dx }ᵈ df -> $ (S x) ∈ᵥ df.
+intros. qual_destruct dx. qual_destruct df. simpl in *. unfold_Q. unfold_q.
+ndestruct (fvs0 0); simpl in *; nlift; unfold_N; intuition. exfalso; eauto.
+Qed.
+
+Lemma subst1_saturated : forall {Γ Σ Tx dx df dx'},
+    saturated (Γ ++ [(Tx, dx)]) Σ df ->
+    closed_Qual 0 0 (length Σ) (Q_lift dx') ->
+    saturated ({0 |-> dx' }ᴳ Γ) Σ ({0 |-> dx' }ᵈ df).
+intros. unfold saturated in *. intros.
+eapply subst1_mem in H1; eauto. apply H in H1. clear H.
+unfold subst_qual,saturated_var in *. qual_destruct df. unfold_q. unfold_Q. destruct H1 as [U [q' H1]]. exists ({0 |-> dx' }ᵀ U),({0 |-> dx' }ᵈ q').
+ndestruct (fvs 0); intuition.
+1,8: eapply @indexr_subst1 with (x:=(S x)); eauto; lia.
+all: qual_destruct q'; qual_destruct dx'; unfold_q; ndestruct (fvs0 0); simpl; nlift; unfold_N; intuition.
+  all: try solve [eauto using lt_S_n]; try solve [exfalso; eauto].
+Qed.
+
+Lemma vtp_closed:
+  forall {Σ t T d}, vtp Σ t T d ->
+    closed_tm 0 0 (length Σ) t /\
+    closed_ty 0 0 (length Σ) T /\
+    closed_Qual 0 0 (length Σ) (Q_lift d).
+Proof.
+  intros. induction H; simpl in *; intuition.
+  - apply indexr_var_some' in H1; intuition.
+  - apply stp_closed in H2. intuition.
+Qed.
+
+Lemma vtp_widening: forall {Σ T1 d1 T2 d2 t},
+  vtp Σ t T1 d1 -> stp ([]: tenv) Σ T1 d1 T2 d2 -> vtp Σ t T2 d2.
+Proof.
+  intros. remember t as tt. remember [] as Γ.  induction H0; subst.
+  - (* vtp_base *)
+    inversion H. subst. econstructor; eauto. apply qstp_closed in H0; intuition.
+  - (* vtp_ref *) inversion H. subst. econstructor; eauto; intuition.
+    + apply qstp_closed in H0; intuition.
+    + eapply s_trans; eauto.
+    + eapply s_trans; eauto.
+    + eapply qstp_trans; eauto.
+  - (* vtp_abs *) inversion H. subst. econstructor; eauto.
+    + apply qstp_closed in H2; intuition.
+    + eapply s_trans; eauto.
+    + eapply qstp_trans; eauto.
+    + assert (stp [] Σ (TFun d1 d2 T1 T2) d5 (TFun d3 d4 T3 T4) d6).
+      { apply s_fun; intuition.  }
+      assert (stp [] Σ (TFun d0 d7 T0 T5) df1 (TFun d1 d2 T1 T2) d5).
+      { apply s_fun; intuition.  }
+      assert (stp [] Σ (TFun d0 d7 T0 T5) df1 (TFun d3 d4 T3 T4) d6).
+      { eapply s_trans; eauto. }
+      assert (stp [] Σ T3 d3 T1 d1). { eauto. }
+      specialize (@narrowing_stp_gen [] T1 d1 [] Σ
+                                     (open_ty' ([]: tenv) T5)(openq' ([]:tenv) d7) (open_ty' ([]:tenv) T2) (openq' ([]: tenv) d2)) as narrow.
+      replace ([] ++ [(T1, d1)]) with [(T1, d1)] in narrow; intuition.
+      simpl in *. apply H11 in H6. clear H11.
+      eapply s_trans; eauto.
+  - intuition.
+Qed.
+
+Lemma has_type_vtp: forall {Σ φ t T d},
+  value t ->
+  has_type [] φ Σ t T d ->
+  vtp Σ t T d.
+Proof.
+  intros. remember [] as Γ.  induction H0; eauto; try inversion H; subst.
+  - (* tabs *) eapply vtp_abs; simpl in *; eauto; intuition.
+    + apply @closed_Qual_sub with (d:=φ); auto.
+    + eapply stp_refl; eauto. unfold_Q; unfold_N; intuition.
+    + unfold_Q; unfold_N; intuition.
+    + eapply stp_refl; eauto. eapply closed_ty_open'; simpl; eauto. unfold_Q; nlift; unfold_N; intuition. unfold openq',openq. constructor; auto. rewrite Q_lift_open_qual. eapply closed_qual_open'; eauto. unfold_Q; nlift; unfold_N; intuition.
+  - (* tloc *) eapply vtp_loc; eauto; intuition.
+    + eapply closed_Qual_sub; eauto.
+    + eapply stp_refl; eauto. unfold_Q; unfold_N; intuition.
+    + eapply stp_refl; eauto. unfold_Q; unfold_N; intuition.
+    + apply Qstp_refl; auto. unfold_Q; unfold_N; intuition.
+  - intuition. eapply vtp_widening; eauto.
+  - intuition. eapply vtp_widening; eauto.
+  - intuition. eapply vtp_widening; eauto.
+Qed.
+
+Lemma vtp_has_type: forall {Σ t T d}, vtp Σ t T d ->  has_type [] d Σ t T d.
+Proof.
+  intros. induction H.
+  - econstructor; eauto. econstructor; eauto. constructor. unfold_Q; unfold_N; intuition. eapply closed_Qual_sub; eauto.
+  - assert (has_type [] (just_loc l) Σ (tloc l) (TRef T) (just_loc l)). { econstructor; eauto. unfold_Q; unfold_N; intuition. }
+    eapply weaken_flt with (φ' := d) in H5; intuition. eapply t_sub; eauto.
+    constructor; intuition. unfold_Q; unfold_N; intuition.
+  - specialize (qstp_closed H5) as Hcl. intuition.
+    assert (has_type [] df1 Σ (tabs t) (TFun d1 d2 T1 T2) df1). {
+    constructor; eauto. apply saturated_empty_tenv. unfold_Q; unfold_N; intuition. }
+    eapply weaken_flt with (φ' := df2) in H9; eauto.
+    eapply t_sub; eauto. constructor; intuition. unfold_Q; unfold_N; intuition.
+Qed.
+
+Lemma narrow_saturated : forall {Γ0 df df' Σ Tx d},
+  df ⊑↑ df' ->
+  saturated (Γ0 ++ [(Tx, df')]) Σ d ->
+  saturated (Γ0 ++ [(Tx, df)]) Σ d.
+intros. unfold saturated,saturated_var in *. intros. specialize (H0 x H1). destruct x; destruct H0 as [U [q' H0]]; intuition.
+  - replace 0 with (length ([] : tenv)) in * by auto. rewrite indexr_insert in H2. inversion H2. clear H2. subst. exists U,df. intuition. rewrite indexr_insert. auto. all: Qcrush.
+  - exists U,q'. intuition. rewrite <- indexr_insert_ge in H2. rewrite <- indexr_insert_ge. auto. all: simpl; lia.
+Qed.
+
+Lemma stp_scale_qor_l : forall {Γ Σ T d1 d2},
+  closed_ty 0 (length Γ) (length Σ) T ->
+  closed_Qual 0 (length Γ) (length Σ) (Q_lift d1) ->
+  closed_Qual 0 (length Γ) (length Σ) (Q_lift d2) ->
+  stp Γ Σ T d2 T (d1 ⊔ d2).
+intros. induction T; constructor; auto.
+1,2: Qcrush. simpl in H. intuition. eapply stp_refl; eauto. Qcrush. unfold open_ty',openq',open_ty,openq. eapply stp_refl; eauto. simpl in H. eapply closed_ty_open'; eauto. intuition. simpl. eapply closed_ty_monotone; eauto. Qcrush. simpl in H. intuition. apply Qstp_refl. simpl. rewrite Q_lift_open_qual. eapply closed_qual_open'; eauto. Qcrush. Qcrush. 1,2: eapply stp_refl; eauto; apply Qstp_refl; Qcrush.
+Qed.
+
+Lemma subst1_Qual_plus' : forall {du du' l},
+    closed_Qual 0 0 l (Q_lift du') -> subst_Qual (Q_lift (du' ⊕ 0)) 0 (Q_lift du) = Qor (Q_lift du') (Q_lift du).
+Proof.
+  intros. qual_destruct du'. qual_destruct du. Qcrush. exfalso. eauto.
+Qed.
+
+Lemma subst1_qual_plus' : forall {du du' l},
+    closed_Qual 0 0 l (Q_lift du') -> subst_qual (du' ⊕ 0) 0 du = (du' ⊔ du).
+Proof.
+  intros. apply Q_lift_eq. apply Q_lift_closed' in H. repeat rewrite Q_lift_subst_qual. erewrite subst1_Qual_plus'. rewrite Q_lift_or. auto. eauto.
+Qed.
+
+Lemma substitution_gen :
+  forall {t Γ φ' Tx dx dx' Σ T d}, dx' ⊓ φ' ⊑↑ dx ->
+    forall {φ}, φ ⊑↑ φ' ->
+      has_type (Γ ++ [(Tx,dx)]) φ Σ t T d -> wf_tenv (Γ ++ [(Tx,dx)]) Σ ->
+        forall {tx}, vtp Σ tx Tx dx' ->
+                        has_type ({ 0 |-> dx' }ᴳ Γ) ({ 0 |-> dx' }ᵈ φ) Σ
+                                 ({ 0 |-> tx  }ᵗ t)
+                                 ({ 0 |-> dx' }ᵀ T)
+                                 ({ 0 |-> dx' }ᵈ d).
+  intros t Γ φ' Tx dx dx' Σ T d Hsep φ Hphi HT HwfG tx HTx. specialize (vtp_closed HTx) as Hclx.
+  simpl in Hclx. intuition. remember (Γ ++ [(Tx, dx)]) as Γ'.
+  generalize dependent Γ. generalize dependent φ'.
+  induction HT; intros; subst; pose (φs := {0 |-> dx' }ᵈ φ); replace ({0 |-> dx' }ᵈ φ) with φs in *; auto.
+  - simpl. replace ({0 |-> dx' }ᵈ ∅) with (∅) by auto.
+    apply t_base; auto. eapply closed_qual_subst1'; eauto.
+  - simpl. bdestruct (x =? 0).
+    + (*x is 0 *) rewrite indexr_skips in H0; simpl; auto; try lia. simpl in H0. subst. simpl in H0.
+      inversion H0. subst. erewrite subst1_ty_id; eauto.
+      apply vtp_has_type in HTx. erewrite subst1_qual_plus'; eauto.
+      apply t_sub with (T1:=T) (d1:=dx').
+      eapply @weaken_flt with (φ:=dx'); eauto.
+      eapply weaken; eauto.
+      subst φs. qual_destruct φ. assert (N_lift fvs 0). { Qcrush. }
+      unfold subst_qual. unfold_q. destruct (fvs 0) eqn:Eq. Qcrush. unfold N_lift in H7. rewrite H7 in Eq. discriminate.
+      subst φs. rewrite subst1_tenv_length. rewrite app_length in H4. simpl in H4. rewrite <- plus_n_Sm in H4. rewrite Nat.add_0_r in H4. eapply closed_Qual_subst1; eauto.
+      apply stp_scale_qor_l; eauto. eapply closed_ty_monotone; eauto; lia. 1,2: eapply closed_Qual_monotone; eauto; lia.
+      subst φs. apply @subst1_Qual_subq with (du':=dx') in H3. eapply @Subq_trans with (d2:={0 |-> dx' }ᵈ (d ⊕ 0)); eauto. erewrite subst1_qual_plus'; eauto.
+      apply saturated_qor; eapply saturated_closed_Qual; eauto.
+    + (* x is in Γ0 *) assert (Hx: 1 <= x); try lia. destruct x; try lia.
+      rewrite subst1_qual_plus_dist; auto. apply t_var; auto.
+      eapply indexr_subst1; eauto. rewrite <- subst1_qual_plus_dist; auto.
+      repeat apply subst_qual_subqual_monotone. auto.
+      eapply closed_qual_subst1'; eauto. simpl. eapply closed_ty_subst1; eauto.
+      simpl. eapply closed_Qual_subst1; eauto.
+  - simpl.
+    (* assert (HwfG' : wf_tenv ((T1, d1) :: Γ0 ++ [(Tx, dx)]) Σ). apply wf_tenv_cons; auto. *)
+    assert (HwfG' : wf_tenv ((T1, d1) :: Γ0 ++ [(Tx, dx)]) Σ). apply wf_tenv_cons; auto.
+    intuition. rename H8 into IHHT.
+    apply t_abs; auto. eapply closed_tm_subst1'; eauto.
+    inversion H3. subst. constructor; intuition; try eapply closed_ty_subst1'; eauto; eapply closed_qual_subst1'; eauto.
+    eapply closed_qual_subst1'; eauto. apply subst_qual_subqual_monotone. auto.
+    1,2 : eapply subst1_saturated; eauto.
+    (* 1. instantiate the IH *)
+    replace (length (Γ0 ++ [(Tx, dx)])) with (S (length Γ0)) in IHHT.
+    rewrite subst1_tenv_length. rewrite app_comm_cons in IHHT. (*  rewrite app_comm_cons in IHHT. *)
+    remember (df ⊔ just_fv (S (length Γ0))) as DF.
+    replace ({0 |-> dx' }ᵈ df ⊔ just_fv (length Γ0)) with ({0 |-> dx' }ᵈ DF).
+    specialize IHHT with (φ' := φ' ⊔ just_fv (S (length Γ0))) (Γ := (((T1, d1) :: Γ0))).
+    (* 2. reason about opening and subst, apply IH *)
+    unfold open_tm' in *. unfold open_ty' in *. unfold open_ty in *.
+    unfold openq' in *. unfold openq in *.
+    rewrite app_length in IHHT. rewrite subst1_tenv_length.
+simpl in *.
+    replace (length Γ0 + 1) with (S (length Γ0)) in IHHT; try lia.
+    erewrite <- open_subst1_tm_comm in IHHT; eauto.
+    erewrite <- open_subst1_ty_comm in IHHT; eauto.
+    erewrite <- open_subst1_qual_comm in IHHT; eauto.
+rewrite qand_qor_dist_l in IHHT. replace (dx' ⊓ $$ (S (length Γ0))) with (∅) in IHHT.
+rewrite qor_empty_right in IHHT. subst.
+assert (df ⊔ $$ (S (length Γ0)) ⊑↑ φ' ⊔ $$ (S (length Γ0))). Qcrush.
+    apply IHHT; auto.
+    (* done, prove some leftovers *)
+apply Q_lift_eq. Qcrush. eauto.
+    subst. apply Q_lift_eq. rewrite subst1_qor_dist. Qcrush.
+    rewrite app_length. simpl. lia.
+  - intuition. rename H7 into IHHT2. rename H5 into IHHT1. simpl.
+    replace ({ 0 |-> dx' }ᵈ (openq d1 d2)) with (openq ({ 0 |-> dx' }ᵈ d1) ({ 0 |-> dx' }ᵈ d2)).
+    (* separation/overap is preserved after substitution *)
+    assert (Hoverlap: {0 |-> dx' }ᵈ (df ⊓ d1) = {0 |-> dx' }ᵈ df ⊓ {0 |-> dx' }ᵈ d1). {
+      specialize (has_type_filter HT1). specialize (has_type_filter HT2).
+      specialize (has_type_saturated HwfG HT1). specialize (has_type_saturated HwfG HT2). intros.
+      symmetry. eapply @subst1_preserves_separation with (φ:=φ'); eauto.
+      all: eapply @narrow_saturated with (df:=(dx' ⊓ φ')); eauto.
+    }
+    apply t_app with (T1:= { 0 |-> dx' }ᵀ T1) (df:=({0 |-> dx' }ᵈ df)).
+    replace (TFun ({0 |-> dx' }ᵈ df ⊓ {0 |-> dx' }ᵈ d1) ({0 |-> dx' }ᵈ d2) ({0 |-> dx' }ᵀ T1) ({0 |-> dx' }ᵀ T2))
+            with ({ 0 |-> dx' }ᵀ (TFun (df ⊓ d1) d2 T1 T2)).
+    eapply IHHT1; eauto. simpl. f_equal. apply Hoverlap.
+    eapply IHHT2; eauto.
+    2,3 : unfold openq; rewrite <- @subst1_qual_empty with (dx:=dx'); erewrite <- subst1_open_qual_comm; eauto.
+    + eapply closed_ty_subst1'; eauto.
+    + apply subst_qual_subqual_monotone. unfold openq in H4. auto.
+    + eapply subst1_saturated; eauto.
+    + unfold openq. repeat erewrite <- subst1_open_qual_comm; eauto.
+  - erewrite @subst1_qual_id with (q:=(just_loc l)); eauto. simpl. erewrite subst1_ty_id; eauto.
+    apply t_loc; auto. eapply closed_qual_subst1'; eauto.
+    subst φs. qual_destruct φ. qual_destruct dx'. unfold_q.
+    ndestruct (fvs 0); simpl in *; unfold_Q; nlift; unfold_N; intuition.
+    unfold_Q; nlift; unfold_N; intuition.
+  - replace ({0 |-> dx' }ᵈ ∅) with (∅) in * by auto.
+    replace ({0 |-> dx' }ᵀ (TRef TUnit)) with (TRef TUnit) in * by auto.
+    replace ({0 |-> dx' }ᵀ (TUnit)) with (TUnit) in * by auto.
+    eapply t_ref. fold subst_tm. eapply IHHT; eauto.
+  - simpl. rewrite subst1_qual_empty.
+    apply t_deref with (d := { 0 |-> dx' }ᵈ d). eapply IHHT; eauto.
+  - replace ({0 |-> dx' }ᵈ ∅) with (∅) in * by auto.
+    replace ({0 |-> dx' }ᵀ (TRef TUnit)) with (TRef TUnit) in * by auto.
+    replace ({0 |-> dx' }ᵀ (TUnit)) with (TUnit) in * by auto.
+    eapply t_assign; eauto.
+  - apply t_sub with (T1:={ 0 |-> dx' }ᵀ T1) (d1:={ 0 |-> dx' }ᵈ d1).
+    eapply IHHT; eauto. eapply subst_stp; eauto. apply subst_qual_subqual_monotone; auto.
+    eapply subst1_saturated; eauto.
+    Unshelve. all : auto.
+Qed.
+
+Lemma open_Qual_mono : forall {d1 d1' d2 k}, d1 ⊑↑ d1' -> ([[ k ~> d1 ]]ᵈ d2) ⊑↑ ([[ k ~> d1' ]]ᵈ d2).
+  intros. repeat rewrite Q_lift_open_qual. Qcrush.
+Qed.
+
+Lemma open_qual_mono : forall {d1 d1' d2 k}, d1 ⊑ d1' -> ([[ k ~> d1 ]]ᵈ d2) ⊑ ([[ k ~> d1' ]]ᵈ d2).
+  intros. apply Q_lift_subq. apply Q_lift_subq' in H. apply open_Qual_mono. auto.
+Qed.
+
+Lemma open_Qual_mono2 : forall {d1 d2 d2' k}, d2 ⊑↑ d2' -> ([[ k ~> d1 ]]ᵈ d2) ⊑↑ ([[ k ~> d1 ]]ᵈ d2').
+  intros. repeat rewrite Q_lift_open_qual. Qcrush. all: nlem; intuition eauto 3.
+Qed.
+
+Lemma open_qual_mono2 : forall {d1 d2 d2' k}, d2 ⊑ d2' -> ([[ k ~> d1 ]]ᵈ d2) ⊑ ([[ k ~> d1 ]]ᵈ d2').
+  intros. apply Q_lift_subq. apply Q_lift_subq' in H. apply open_Qual_mono2. auto.
+Qed.
+
+Lemma openq_mono : forall {d1 d1' d2 d2' f l},
+  closed_qual 0 f l d1' -> d1 ⊑ d1' -> d2 ⊑ d2' -> (openq d1 d2) ⊑ (openq d1' d2').
+  intros. unfold openq.
+  specialize (@open_qual_mono d1 d1' d2' 0 H0) as S1.
+  specialize (@open_qual_mono2 d1 d2 d2' 0 H1) as S2.
+  eapply subq_trans; eauto.
+Qed.
+
+Lemma stp_scale_qor : forall {Γ Σ T1 d1 T2 d2}, stp Γ Σ T1 d1 T2 d2 -> forall {d}, closed_Qual 0 (length Γ) (length Σ) (Q_lift d) -> stp Γ Σ T1 (d1 ⊔ d) T2 (d2 ⊔ d).
+  intros Γ Σ T1 d1 T2 d2 HSTP. induction HSTP; intros.
+  - inversion H. constructor. constructor.
+    apply Subq_qor; auto. apply closed_qual_qor; auto.
+  - inversion H. constructor; auto. constructor.
+    apply Subq_qor; auto. apply closed_qual_qor; auto.
+  - inversion H1. constructor; auto. constructor. apply Subq_qor; auto. apply closed_qual_qor; auto.
+  - econstructor; auto.
+Qed.
+
+Lemma open_qual_qor_dist : forall {k d1 d2 d3}, ([[ k ~> d1  ]]ᵈ (d2 ⊔ d3)) = (([[ k ~> d1  ]]ᵈ d2) ⊔ ([[ k ~> d1  ]]ᵈ d3)).
+  intros. apply Q_lift_eq. qual_destruct d2. qual_destruct d3. qual_destruct d1. rewrite Q_lift_or,Q_lift_open_qual. unfold_q.
+ndestruct (bvs k); ndestruct (bvs0 k); Qcrush.
+all: intuition eauto.
+Qed.
+
+Lemma openq_u_distribute: forall {d1 d2 d3 : qual}, openq d1 (d2 ⊔ d3) = (openq d1 d2 ⊔ openq d1 d3).
+  intros. unfold openq. repeat rewrite open_qual_qor_dist. auto.
+Qed.
+
+Lemma openq_u_distribute1 : forall {d1 d2 l},
+    openq d1 (d2 ⊔ (just_loc l)) = ((openq d1 d2) ⊔ (just_loc l)).
+  intros. unfold openq. rewrite open_qual_qor_dist. auto.
+Qed.
+
+Lemma openq_duplicate_eq : forall {d1 d2 l},
+    (((openq (d1 ⊔ (just_loc l)) d2) ⊔ (just_loc l)) = ((openq d1 d2) ⊔ (just_loc l))).
+intros. unfold openq. qual_destruct d2. qual_destruct d1. apply Q_lift_eq. unfold_q.
+ndestruct (bvs 0); unfold_Q; nlift; unfold_N; repeat f_equal; apply functional_extensionality; intros; apply propositional_extensionality; intuition.
+Qed.
+
+Lemma freshness : forall {Σ Σ' l b f d1}, disjointq Σ Σ' (just_loc l) -> closed_Qual b f (length Σ) (Q_lift d1) -> just_loc l ⊓ d1 = ∅.
+  intros. inversion H; subst. unfold_q. unfold just_loc in H1.
+  inversion H1. apply N_lift_eq' with (x:=l) in H3. Qcrush.
+  inversion H3. apply N_lift_eq' with (x:=l) in H5. apply Q_lift_eq. rewrite Q_lift_and. Qcrush. subst. eauto.
+Qed.
+
+Lemma just_loc_ldom : forall {l} {Σ : senv}, l < length Σ -> just_loc l ⊑↑ qdom Σ.
+  intros. unfold qdom. unfold_Q. nlift. unfold_N. intuition.
+Qed.
+
+Lemma vtp_canonical_form_loc : forall {Σ t T d},
+   vtp Σ t (TRef T) d -> value t -> exists (l : loc), t = tloc l.
+Proof.
+  intros. remember (TRef T) as R. remember t as tt. generalize dependent T.
+  induction H; intuition; try discriminate; inversion H0; subst. exists l. intuition.
+Qed.
+
+Lemma vtp_canonical_form_lam : forall {Σ t T1 T2 d1 d2 df},
+    vtp Σ t (TFun d1 d2 T1 T2) df -> value t -> exists (t' : tm), t = tabs t'.
+Proof.
+  intros Σ t T1 T2 d1 d2 df H. remember (TFun d1 d2 T1 T2) as T.
+  generalize dependent d1. generalize dependent d2. generalize dependent T1. generalize dependent T2.
+  induction H; intuition; try discriminate; inversion H0; subst. exists t. intuition.
+Qed.
+
+Lemma substitution : forall {t df Tx dx dx' Σ T d},
+    has_type [(Tx,dx')] (df ⊔ (just_fv 0)) Σ t T d ->
+    wf_tenv [(Tx,dx')] Σ ->
+    df ⊓ dx ⊑↑ dx' ->
+    closed_Qual 0 0 (length Σ) (Q_lift df) ->
+            forall {vx}, vtp Σ vx Tx dx ->
+                    has_type [] (df ⊔ dx) Σ
+                             ({ 0 |-> vx }ᵗ t)
+                             ({ 0 |-> dx }ᵀ T)
+                             ({ 0 |-> dx }ᵈ d).
+  intros t df Tx dx dx' Σ T d H Hwf Hsub Hcl vx Hvtp. intros. specialize (vtp_closed Hvtp) as Hclx. specialize (has_type_closed H) as Hclt.
+  intuition. replace ([(Tx, dx')]) with ([] ++ [(Tx, dx')]) in H; auto.
+  remember (df ⊔ (just_fv 0)) as DF.
+  assert (Hsepf : dx ⊓ (df ⊔ just_fv 0) ⊑ dx'). {
+    rewrite qand_qor_dist_l. replace (dx ⊓ $$ 0) with (∅). rewrite qor_empty_right. rewrite qand_commute. auto. apply Q_lift_eq. Qcrush. eauto.
+  }
+  assert (Hrefl : DF ⊑↑ DF). unfold_Q; unfold_N; intuition. subst DF.
+replace ([(Tx, dx')]) with ([] ++ [(Tx, dx')]) in H by auto.
+  eapply (substitution_gen Hsepf Hrefl) in H; eauto.
+  replace ({0 |-> dx }ᵈ (df ⊔ just_fv 0)) with (df ⊔ dx) in H. apply H.
+  (* done, prove earlier replacements *)
+  rewrite subst1_qor_dist. rewrite subst1_just_fv0. erewrite subst1_qual_id; eauto.
+Qed.
+
+(* Main results: type soundness & preservation of separation *)
+
+Theorem type_safety: forall {Σ t T d},
+  has_type [] (qdom Σ) Σ t T d ->
+    value t \/
+    forall {σ} , CtxOK [] (qdom Σ) Σ σ ->
+    exists t' σ', step t σ t' σ' /\ preserve [] Σ t' T d σ'.
+Proof.
+  intros Σ t T d H.
+  specialize (has_type_closed H) as HX. remember [] as G. remember t as tt. remember T as TT. remember (qdom Σ) as φ.
+  revert T t HeqTT Heqtt HeqG Heqφ.
+  induction H; try (left; constructor); intros.
+  - (* tvar *)  subst. inversion H.
+  - (* tapp *) right. subst. intuition.
+    apply has_type_closed in H as HH. intuition. apply has_type_closed in H0 as HH0. intuition.
+    (* t1 *) specialize (H7 (TFun (df ⊓ d1) d2 T1 T) t1).  intuition.
+    (* t2 *) specialize (H9 T1 t2). intuition.
+    + (* beta *)
+      (* turn has_type to vtp *)
+      apply has_type_vtp in H as VH; intuition.
+      pose (VHH := VH). inversion VH. subst.
+      specialize (has_type_filter H0) as Hflt0.
+      apply has_type_vtp in H0 as VH0; intuition.
+      exists (open_tm  t2 t). exists σ. intuition.
+      * constructor. intuition.
+      * apply (Preserve Σ ∅); auto. rewrite qor_empty_right.
+        apply qstp_closed in H32 as H32'; intuition.
+        apply stp_qstp_inv in H31 as H31'. unfold Qstp in H31'. intuition.
+        apply Q_lift_subq in H21.
+
+        change (length []) with 0 in *. subst.
+        assert (HT' : has_type [(T0, d0)] (df ⊔ just_fv 0) Σ (open_tm' ([]:tenv) t) (open_ty' ([]:tenv) T2) (openq' ([]:tenv) d3)). {
+          eapply weaken_flt; eauto. unfold_Q; nlift; unfold_N; intuition.
+        }
+        eapply @substitution  with ( vx:= t2) (dx:=d1)  in HT' as HT''; eauto; intuition.
+        unfold open_tm' in HT''. unfold open_ty' in HT''. unfold openq' in HT''. simpl in HT''. inversion H26; subst.
+        unfold open_ty in HT''. unfold openq in HT''.
+        erewrite <- open_subst1_tm in HT''; eauto. erewrite <- open_subst1_qual in HT''; eauto. erewrite <- open_subst1_ty in HT''; eauto.
+        fold (open_tm t2 t) in HT''. fold (openq d1 d3) in HT''.
+        apply @weaken_flt with (φ':= (qdom Σ)) in HT''; auto; intuition.
+        eapply t_sub; eauto.
+        simpl in *. rename H33 into Hsub.
+        eapply @subst_stp with (Γ := [])(df' := d1) in Hsub; eauto.
+        replace (open_ty' ([] : tenv) T) with T in *. (* because T is closed *)
+        simpl in Hsub. unfold openq' in Hsub. unfold openq in Hsub. simpl in Hsub.
+        erewrite @subst1_ty_id with (T := T) in Hsub; eauto.
+        unfold open_ty' in Hsub. unfold open_ty in Hsub.
+        erewrite <- open_subst1_ty in Hsub; eauto.
+        erewrite <- open_subst1_qual in Hsub; eauto.
+        erewrite <- open_subst1_qual in Hsub; eauto.
+        Qcrush.
+        unfold open_ty'. unfold open_ty. repeat erewrite closed_ty_open_id; eauto.
+        unfold openq. intuition. eapply openq_subqual; auto.
+        apply qor_bound; auto. apply has_type_filter in H. auto.
+        intuition eauto.
+        intuition eauto.
+        apply wf_tenv_cons; auto.
+        eapply vtp_widening; eauto.
+        eapply stp_refl_qual; eauto.
+    + (* (tabs t) t2 -> (tabs t) t2' *)
+      apply has_type_vtp in H as VH; intuition.
+      apply vtp_canonical_form_lam in VH as HH; intuition.
+      pose (HH10 := H10).
+      unfold CtxOK in HH10. specialize (H7 σ). intuition.
+      destruct H21 as [t2' [σ' HH21]]. exists (tapp t1 t2'). exists σ'. intuition. constructor; intuition.
+      destruct H21.  apply (Preserve Σ' d'); intuition.
+      inversion H23; subst.
+      * rewrite qor_empty_right. rewrite qor_empty_right in H24. eapply t_app with (df := df); eauto.
+        eapply weaken_flt. eapply weaken_store; eauto; intuition. apply extends_ldom. auto.
+        apply extends_length in H21. unfold_Q; erewrite N_lift_dom; unfold_N; intuition.
+        eapply closed_ty_monotone; eauto. apply extends_length. intuition.
+        Qcrush.
+        apply extends_length in H21. unfold_N. eauto 4 using Nat.lt_le_trans.
+        eapply weaken_store_saturated; eauto.
+      * specialize (has_type_closed H). specialize (has_type_closed H24). intuition. simpl in H32. intuition. rewrite <- openq_duplicate_eq.
+        apply t_sub with (T1 := T) (d1 := (openq (d1 ⊔ (just_loc l)) d2)).
+        -- eapply t_app with (T1 := T1) (df:=df); eauto. erewrite <- qand_fresh_r; eauto. eapply weaken_flt. eapply weaken_store; eauto.
+           apply extends_ldom. auto. simpl. auto.
+           eapply Subq_trans; eauto. apply extends_ldom; auto.
+           eapply weaken_store_saturated; eauto.
+        -- eapply stp_refl; eauto. unfold openq. simpl. repeat rewrite Q_lift_or,Q_lift_open_qual,Q_lift_or. clear - H25 H26 H32 H33 H35 H34. Qcrush. nlem; intuition. nlem; intuition. eapply closed_Nats_tighten; eauto. nlem; intuition eauto 4 using Nat.le_lt_trans,Nat.lt_trans.
+        -- apply has_type_filter in H0. apply qor_bound. apply openq_subqual. apply qor_bound.
+           1, 3 : eapply Subq_trans; eauto; apply extends_ldom; auto. all : apply just_loc_ldom; auto.
+        -- apply saturated_qor; auto. apply saturated_openq. apply saturated_qor; auto.
+           apply saturated_empty_tenv. eapply closed_Qual_monotone; eauto. lia. eapply weaken_store_saturated; eauto.
+    + (*  t t2 -> t' t2  *)
+      apply has_type_closed in H0 as Hcl. intuition.
+      specialize (H18 σ H10). destruct H18 as [t1' [σ' HH5]]. exists (tapp t1' t2). exists σ'. intuition. apply step_c_app_l. intuition.
+      destruct H22. apply (Preserve Σ' d'); intuition. inversion H25; subst.
+      * rewrite qor_empty_right. rewrite qor_empty_right in H26. eapply t_app; eauto.
+        eapply weaken_flt. eapply weaken_store; eauto. apply extends_ldom. auto. Qcrush.
+        eapply closed_ty_monotone; eauto. apply extends_length. auto.
+        eapply Subq_trans; eauto; apply extends_ldom; auto.
+        eapply weaken_store_saturated; eauto.
+      * rewrite <- openq_u_distribute1. eapply t_sub with (T1 := T)(d1 := (openq d1 d2)).
+        -- eapply t_app with (df:=(df ⊔ just_loc l)); eauto. erewrite <- qand_fresh_l; eauto.
+           eapply weaken_flt. eapply weaken_store. eauto. auto. apply extends_ldom; auto. Qcrush.
+           eapply Subq_trans; eauto. apply extends_ldom; auto. eapply weaken_store_saturated; eauto.
+        -- eapply stp_refl; eauto. simpl.
+           constructor. eapply openq_mono; eauto. apply subq_qor_gt.
+           unfold openq. rewrite Q_lift_open_qual. eapply closed_qual_open'; eauto. simpl in H12. intuition. apply closed_Qual_qor; eauto. Qcrush.
+        -- apply has_type_filter in H0. apply openq_subqual. eapply Subq_trans; eauto. apply extends_ldom. auto.
+           rewrite openq_u_distribute1. apply qor_bound. eapply Subq_trans; eauto. apply extends_ldom. auto.
+           apply just_loc_ldom. auto.
+        -- rewrite openq_u_distribute1. apply saturated_qor; auto. apply saturated_openq. apply saturated_empty_tenv.
+           eapply closed_Qual_monotone; eauto. lia. eapply weaken_store_saturated; eauto.
+  - (* tref *) subst. intuition. specialize (has_type_closed H) as HH. intuition. specialize (H8 TUnit t). intuition.
+    + (* contraction *) right. intros.
+      exists (tloc (length (σ))). exists (t :: σ). intuition.
+      econstructor; eauto. apply (Preserve (TUnit :: Σ) (just_loc (length σ))). apply extends_cons. eapply CtxOK_weaken_flt.
+      apply CtxOK_ext; auto. apply H8.
+      pose (HV := H). apply has_type_vtp in HV; intuition. inversion HV; subst. constructor. auto. Qcrush.
+      Qcrush. simpl. lia. simpl.
+      inversion H8. apply (disj_loc (length σ)); simpl; eauto; lia.
+      replace (∅ ⊔ just_loc (length σ)) with (just_loc (length σ)).
+      inversion H8. rewrite <- H10.
+      eapply t_loc; eauto. Qcrush.
+      apply indexr_head.
+      Qcrush. simpl. lia. Qcrush.
+    + (* congruence *) right. intros. specialize (H5 σ H8). destruct H5 as [t' [σ' HH8]]. exists (tref t'). exists σ'. intuition. econstructor; eauto.
+      destruct H10. apply (Preserve Σ' ∅); intuition. rewrite qor_empty_right. eapply t_ref; eauto.
+  - (* tderef *) subst. intuition. specialize (has_type_closed H) as HH. intuition. specialize (H3 (TRef T0) t). intuition.
+    + (* contraction *) right. intros. pose (HV := H). apply has_type_vtp in HV; intuition.
+      specialize (vtp_canonical_form_loc HV) as Hcan. intuition. destruct H10 as [l HH10]. subst.
+      pose (HHV := HV). inversion HHV. subst.  pose (HH3 := H3). destruct HH3. subst.
+      pose (HH14 := H14). apply indexr_var_some' in HH14. rewrite H10 in HH14. apply indexr_var_some in HH14.
+      destruct HH14 as [v HHH14].  exists v. exists σ. intuition. apply step_deref; intuition.
+      apply (Preserve Σ ∅); intuition.
+      simpl. rewrite qor_empty_right.  apply t_sub with (T1 := T)(d1:= ∅); auto.
+      specialize (H11 l v T). intuition.
+      replace Σ with (Σ ++ []); intuition. eapply weaken_stp_store. auto.
+    + (* congruence *) right. intros. specialize (H8 σ H3).
+      destruct H8 as [t' [σ' HH8]]. exists (tderef t'). exists σ'. intuition. constructor; auto.
+      destruct H10. apply (Preserve Σ' ∅); intuition. simpl. rewrite qor_empty_right. eapply t_deref; eauto.
+  - (* tassign *) subst. intuition. rename H into Ht1. rename H0 into Ht2. intuition.
+    apply has_type_closed in Ht1 as Ht1C. intuition.
+    apply has_type_closed in Ht2 as Ht2C. intuition.
+    specialize (H4 (TRef TUnit) t1). intuition.
+    specialize (H6 TUnit t2). intuition.
+    + (* contraction *)
+      right. intros.
+      pose (Ht1' := Ht1). eapply has_type_vtp in Ht1'; eauto.
+      pose (Hloc := Ht1'). apply vtp_canonical_form_loc in Hloc; auto.
+      inversion Ht1'. destruct Hloc. subst.
+      pose (Ht2' := Ht2). apply has_type_vtp in Ht2'; auto.
+      inversion Ht2'. subst.
+      exists tunit. exists (update σ x tunit). inversion H21. subst.
+      simpl in  H7. inversion H6. subst. intuition.
+      econstructor; eauto. lia. apply (Preserve Σ ∅); auto.
+      eapply CtxOK_update; eauto. lia. apply t_sub with (T1:=TUnit) (d1:=∅); auto.
+      replace Σ with (Σ ++ []); intuition. eapply weaken_stp_store. auto.
+    + (* right congruence *)
+      right. intros. specialize (H4 σ H6). destruct H4 as [t' [σ' H4']].
+      exists (tassign t1 t'). exists σ'. intuition. econstructor; eauto.
+      pose (HV := Ht1). apply has_type_vtp in HV; intuition. inversion HV; subst.
+      destruct H14. apply (Preserve Σ' ∅); eauto. simpl. rewrite qor_empty_right.
+      eapply t_assign; eauto.
+      assert (qdom Σ ⊑ qdom Σ'). apply extends_ldom. auto.
+      eapply weaken_store in Ht1; eauto. eapply weaken_flt in Ht1; eauto. Qcrush.
+    + (* left congruence *)
+      right. intros. specialize (H12 σ H4). destruct H12 as [t' [σ' H12']].
+      exists (tassign t' t2). exists σ'. intuition. econstructor; eauto.
+      destruct H14. apply (Preserve Σ' ∅); eauto. simpl. rewrite qor_empty_right.
+      eapply t_assign; eauto. eapply weaken_store in Ht2; eauto. eapply weaken_flt; eauto. apply extends_ldom; auto. Qcrush.
+  - (* subsumption *) subst. intuition. specialize (stp_closed H0) as H00. intuition.
+    specialize (H6 T1 t). intuition. right.
+    intros. specialize (H11 σ H6). destruct H11 as [t' [σ' HH9]]. exists t'. exists σ'. intuition.
+    destruct H13. apply (Preserve Σ' d'); intuition. eapply t_sub; eauto. apply stp_scale_qor.
+    eapply weaken_stp_store_ext; eauto. apply extends_length in H13. inversion H15; subst; intuition. Qcrush.
+    apply qor_bound. eapply Subq_trans; eauto. apply extends_ldom; auto. inversion H15; subst; auto.
+    apply just_loc_ldom; auto. apply saturated_qor. eapply weaken_store_saturated; eauto.
+    inversion H15; subst; auto.
+Qed.
+
+Lemma step_deterministic:  deterministic step.
+  unfold deterministic. intros t t1 t2 σ σ1 σ2 Hstep1 Hstep2. generalize dependent σ2. generalize dependent t2.
+  induction Hstep1; intros; inversion Hstep2; subst; auto; try solve [match goal with
+  | [ H : step _ _ _ _  |- _ ] => eapply values_stuck in H; eauto; contradiction (* stuck cases, contradiction *)
+  | [ H1 : step ?t ?s ?t' ?s', (* congruence cases, use IH *)
+      IH : forall _ _, step ?t ?s _ _ -> _ |- _ = _ /\ _ = ?s' ] => specialize (IH t' s'); intuition; f_equal; auto
+  end].
+  rewrite H1 in H. inversion H. subst. intuition.
+Qed.
+
+Lemma progress : forall {Σ t T d},
+    has_type [] (qdom Σ) Σ t T d ->
+    value t \/ forall {σ}, CtxOK [] (qdom Σ) Σ σ -> exists t' σ', step t σ t' σ'.
+Proof.
+  intros Σ t T d HT.
+  specialize (type_safety HT). intuition. right. intros σ HCtxOK.
+  specialize (H0 σ HCtxOK). destruct H0 as [t' [σ' [Hstep  HPreserve]]].
+  exists t'. exists σ'. intuition.
+Qed.
+
+Lemma preservation : forall {Σ t T d},
+    has_type [] (qdom Σ) Σ t T d ->
+    forall{σ}, CtxOK [] (qdom Σ) Σ σ ->
+    forall {t' σ'}, step t σ t' σ' ->
+    preserve [] Σ t' T d σ'.
+Proof.
+  intros Σ t T d HT σ  HCtxOK t' σ' HStep.  specialize (type_safety HT). intuition.
+  - inversion HStep; subst; inversion H0.
+  - specialize (H0 σ HCtxOK). destruct H0 as [t'' [σ'' [HStep2 HPreserve]]].
+    assert (t'' = t' /\ σ' = σ''). { intuition. 1,2: eapply step_deterministic; eauto.  }
+    intuition. subst. intuition.
+Qed.
+
+Corollary preservation_of_separation : forall {Σ t1 T1 q1 t2 T2 q2},
+  has_type [] (qdom Σ) Σ t1 T1 q1 ->
+  has_type [] (qdom Σ) Σ t2 T2 q2 -> q1 ⊓ q2 ⊑ ∅ ->
+    forall{σ}, CtxOK [] (qdom Σ) Σ σ ->
+      forall {t1' σ'}, step t1 σ t1' σ' ->
+      forall {t2' σ''}, step t2 σ' t2' σ'' -> separate Σ t1' T1 t2' T2.
+  intros Σ t1 T1 q1 t2 T2 q2 HT1 HT2 Hsep σ HOK t1' σ' Hstep1 t2' σ'' Hstep2.
+  (* execute preservation in sequence *)
+  specialize (preservation HT1 HOK Hstep1) as P1. destruct P1 as [Σ' d1 Hext1 HOK' Hdisj1 HT1'].
+  assert (HT2': has_type [] (qdom Σ') Σ' t2 T2 q2). {
+    eapply weaken_flt. eapply weaken_store. eauto. auto. apply extends_ldom; auto. Qcrush. }
+  specialize (preservation HT2' HOK' Hstep2) as P2. destruct P2 as [Σ'' d2 Hext2 HOK'' Hdisj2 HT2''].
+  apply (Separate Σ' Σ'' (q1 ⊔ d1) (q2 ⊔ d2) Hext1 Hext2 HT1' HT2'').
+  (* now we just need to show that the disjointness is preserved. this is intuitively true from the disjointness
+     of the heap effects d1 and d2. *)
+  inversion Hdisj1; inversion Hdisj2; subst. 1-3 : repeat rewrite qor_empty_right; auto.
+  - rewrite qand_qor_dist_l. rewrite (@qand_commute q1 (just_loc l)). erewrite freshness; eauto.
+    rewrite qor_empty_right. auto. apply has_type_closed in HT1. intuition. eapply closed_Qual_monotone; eauto.
+    apply extends_length. auto.
+  - rewrite qand_qor_dist_r. erewrite freshness; eauto. rewrite qor_empty_right. auto.
+    apply has_type_closed in HT2. intuition. eapply closed_Qual_monotone; eauto.
+  - rewrite qand_qor_dist_l. rewrite qand_qor_dist_r. rewrite qand_qor_dist_r.
+    erewrite freshness; eauto. rewrite (@qand_commute (just_loc l) (just_loc l0)).
+    erewrite @freshness with (Σ := Σ'); eauto. repeat rewrite qor_empty_right.
+    rewrite (@qand_commute q1 (just_loc l0)). erewrite freshness; eauto. rewrite qor_empty_right. auto.
+    apply has_type_closed in HT1. 3 : apply has_type_closed in HT2. 1,3: intuition; eapply closed_Qual_monotone; eauto;
+    apply extends_length; auto. Qcrush.
+    Unshelve. all : auto.
+Qed.
